\input{preamble}

\FBOX{
11.3
Solve Equation 11.17 for the case of a {\it time-independent} perturbation,
assuming that $c_a(0)=1$ and $c_b(0)=0$.
Check that $|c_a(t)|^2+|c_b(t)|^2=1$.
}

\begin{equation*}
\dot c_a=-\frac{i}{\hbar}H_{ab}'e^{-i\omega_0t}c_b,\quad
\dot c_b=-\frac{i}{\hbar}H_{ba}'e^{i\omega_0t}c_a
\tag{11.17}
\end{equation*}

Laplace transform:
\begin{align*}
sC_a(s)-c_a(0)&=-\frac{i}{\hbar}H_{ab}'C_b(s+i\omega_0)
\\
sC_b(s)-c_b(0)&=-\frac{i}{\hbar}H_{ba}'C_a(s-i\omega_0)
\end{align*}

Solve for $C_a(s)$.
\begin{equation*}
C_a(s)=\frac{1}{s}\left[-\frac{i}{\hbar}H_{ab}'C_b(s+i\omega_0)+1\right]
\end{equation*}

Hence
\begin{equation*}
C_a(s-i\omega_0)=-\frac{iH_{ab}'C_b(s)}{\hbar(s-i\omega_0)}+\frac{1}{s-i\omega_0}
\end{equation*}

Substitute for $C_a(s-i\omega_0)$ in the equation for $C_b(s)$ to obtain
\begin{equation*}
sC_b(s)=-\frac{i}{\hbar}H_{ba}'\left[-\frac{iH_{ab}'C_b(s)}{\hbar(s-i\omega_0)}+\frac{1}{s-i\omega_0}\right]
\end{equation*}

Rewrite as
\begin{equation*}
sC_b(s)+\frac{H_{ab}'H_{ba}'C_b(s)}{\hbar^2(s-i\omega_0)}=-\frac{iH_{ba}'}{\hbar(s-i\omega_0)}
\end{equation*}

Hence
\begin{equation*}
C_b(s)=-\frac
{\displaystyle\frac{iH_{ba}'}{\hbar(s-i\omega_0)}}
{\displaystyle s+\frac{H_{ab}'H_{ba}'}{\hbar^2(s-i\omega_0)}}
=-\frac{iH_{ba}'/\hbar}{s^2-i\omega_0s+H_{ab}'H_{ba}'/\hbar^2}
\end{equation*}

Inverse Laplace transform:
\begin{equation*}
\frac{1}{s^2+as+b}\quad\Rightarrow\quad
\frac{2}{\omega}\sin\left(\frac{\omega t}{2}\right)\exp\left(-\frac{at}{2}\right),\quad
\omega=\sqrt{4b-a^2}
\end{equation*}

Hence for $a=-i\omega_0$ and $b=H_{ab}'H_{ba}'/\hbar^2$ we have
\begin{equation*}
c_b(t)=-\frac{2iH_{ba}'}{\hbar\omega}
\sin\left(\frac{\omega t}{2}\right)
\exp\left(\frac{i\omega_0t}{2}\right),\quad
\omega=\sqrt{\frac{4H_{ab}'H_{ba}'}{\hbar^2}+\omega_0^2}
\end{equation*}

\end{document}
