\input{preamble}

\FBOX{
10.8
Check that equation 10.65 satisfies Equation 10.52, by direct substitution.
{\it Hint:} $\nabla^2(1/r)=-4\pi\delta^3(\mathbf r)$.
}

Note: $r=|\mathbf r|$
\begin{gather*}
\left(\nabla^2+k^2\right)G(\mathbf r)=\delta^3(\mathbf r)\tag{10.52}
\\
G(\mathbf r)=-\frac{e^{ikr}}{4\pi r}\tag{10.65}
\end{gather*}

Recall $\nabla^2=\nabla\cdot\nabla$ and
\begin{equation*}
\nabla\cdot(f\mathbf A)=\nabla f\cdot\mathbf A+f\nabla\mathbf\cdot\mathbf A
\end{equation*}

Hence
\begin{align*}
\nabla^2G(\mathbf r)&=-\frac{1}{4\pi}\nabla\cdot\nabla\left(\frac{e^{ikr}}{r}\right)
\\
&=-\frac{1}{4\pi}\nabla\cdot\left(\frac{1}{r}\nabla e^{ikr}+e^{ikr}\nabla\frac{1}{r}\right)
\\
&=-\frac{1}{4\pi}\biggl(
\underset{\text{see (2)}}{\nabla\frac{1}{r}\cdot\nabla e^{ikr}}
+\underset{\text{see (3)}}{\frac{1}{r}\nabla^2e^{ikr}}
+\underset{\text{see (2)}}{\nabla e^{ikr}\cdot\nabla\frac{1}{r}}
+e^{ikr}\nabla^2\frac{1}{r}
\biggr)\tag{1}
\end{align*}

In spherical coordinates
\begin{equation*}
\nabla\frac{1}{r}\cdot\nabla e^{ikr}
=\begin{pmatrix}-1/r^2\\0\\0\end{pmatrix}
\cdot\begin{pmatrix}ike^{ikr}\\0\\0\end{pmatrix}
=-\frac{ike^{ikr}}{r^2}\tag{2}
\end{equation*}

and
\begin{align*}
\frac{1}{r}\nabla^2e^{ikr}&=\frac{1}{r^2}\frac{\partial^2}{\partial r^2}(re^{ikr})
\\
&=\frac{1}{r^2}\frac{\partial}{\partial r}\left(e^{ikr}+ikre^{ikr}\right)
\\
&=\frac{1}{r^2}\left(2ike^{ikr}-k^2re^{ikr}\right)
\\
&=\frac{2ike^{ikr}}{r^2}-\frac{k^2e^{ikr}}{r}\tag{3}
\end{align*}

Substitute into (1) to obtain
\begin{align*}
\nabla^2G(\mathbf r)&=\frac{k^2e^{ikr}}{4\pi r}-\frac{1}{4\pi}e^{ikr}\nabla^2\frac{1}{r}
\\
&=-k^2G(\mathbf r)+\delta^3(\mathbf r)e^{ikr}
\end{align*}

Noting that $e^{ikr}=1$ for $r=0$ we have
\begin{equation*}
\nabla^2G(\mathbf r)=-k^2G(\mathbf r)+\delta^3(\mathbf r)\tag{4}
\end{equation*}

\end{document}
