\input{preamble}

\FBOX{
11.5
Suppose you {\it don't} assume $H_{aa}'=H_{bb}'=0$.

(a) Find $c_a(t)$ and $c_b(t)$ in first-order perturbation theory,
for the case $c_a(0)=1$, $c_b(0)=0$.
Show that $\bigl|c_a^{(1)}\bigr|^2+\bigl|c_b^{(1)}\bigr|^2=1$, to first order in $\hat H'$.

(b) There is a nicer way to handle this problem. Let
\begin{equation*}
d_a\equiv e^{\frac{i}{\hbar}\int_0^tH_{aa}'(t')\,dt'}c_a,\quad
d_b\equiv e^{\frac{i}{\hbar}\int_0^tH_{bb}'(t')\,dt'}c_b.
\tag{11.26}
\end{equation*}

Show that
\begin{equation*}
\dot d_a=-\frac{i}{\hbar}e^{i\phi}H_{ab}'e^{-i\omega_0t}d_b;\quad
\dot d_b=-\frac{i}{\hbar}e^{-i\phi}H_{ba}'e^{i\omega_0t}d_a.
\tag{11.27}
\end{equation*}

where
\begin{equation*}
\phi(t)\equiv\frac{i}{\hbar}\int_0^t
\left[H_{aa}'(t')-H_{bb}'(t')\right]dt'.
\tag{11.28}
\end{equation*}

So the equations for $d_a$ and $d_b$ are identical in structure to
Equation 11.17 (with an extra factor $e^{i\phi}$ tacked onto $\hat H'$).

(c) Use the method in part (b) to obtain $c_a(t)$ and $c_b(t)$ in first-order
perturbation theory, and compare your answer to (a).
Comment on any discrepancies.
}

(a) From equations (11.14) and (11.15)
\begin{equation*}
\begin{aligned}
\dot c_a&=-\frac{i}{\hbar}\left(c_aH_{aa}'+c_bH_{ab}'e^{-i\omega_0t}\right)
\\
\dot c_b&=-\frac{i}{\hbar}\left(c_bH_{bb}'+c_aH_{ba}'e^{i\omega_0t}\right)
\end{aligned}
\tag{1}
\end{equation*}

Zeroth order:
\begin{equation*}
c_a(t)=1,\quad c_b(t)=0
\end{equation*}

First order:
\begin{align*}
\dot c_a^{(1)}&=-\frac{i}{\hbar}\left[c_aH_{aa}'+c_bH_{ab}'e^{-i\omega_0t}\right]_{c_a=1,c_b=0}
&&=-\frac{i}{\hbar}H_{aa}'
\\
\dot c_b^{(1)}&=-\frac{i}{\hbar}\left[c_bH_{bb}'+c_aH_{ba}'e^{i\omega_0t}\right]_{c_a=1,c_b=0}
&&=-\frac{i}{\hbar}H_{ba}'e^{i\omega_0t}
\end{align*}

Hence
\begin{align*}
c_a^{(1)}&=1-\frac{i}{\hbar}\int_0^tH_{aa}'(t')\,dt'
\\
c_b^{(1)}&=0-\frac{i}{\hbar}\int_0^tH_{ba}'(t')e^{i\omega_0t'}\,dt'
\end{align*}

Hence to first order (discard $|H_{aa}'|^2$ and $|H_{ba}'|^2$)
\begin{align*}
\bigl|c_a^{(1)}\bigr|^2&=1+\left[-\frac{i}{\hbar}\int_0^tH_{aa}'(t')\,dt'\right]
\left[-\frac{i}{\hbar}\int_0^tH_{aa}'(t')\,dt'\right]^*
& {}&=1
\\
\bigl|c_b^{(1)}\bigr|^2&=\left[-\frac{i}{\hbar}\int_0^tH_{ba}'(t')e^{i\omega_0t'}\,dt'\right]
\left[-\frac{i}{\hbar}\int_0^tH_{ba}'(t')e^{i\omega_0t'}\,dt'\right]^*
& {}&=0
\end{align*}

(b) Let
\begin{equation*}
A=\frac{i}{\hbar}\int_0^tH_{aa}'(t')\,dt',\quad
B=\frac{i}{\hbar}\int_0^tH_{bb}'(t')\,dt'
\end{equation*}

so that
\begin{equation*}
d_a=e^Ac_a,\quad d_b=e^Bc_b
\tag{2}
\end{equation*}

For time derivatives we have
\begin{align*}
\dot d_a&=\frac{de^A}{dt}c_a+e^A\dot c_a&&=\frac{i}{\hbar}H_{aa}'e^Ac_a+e^A\dot c_a
\\
\dot d_b&=\frac{de^B}{dt}c_b+e^B\dot c_b&&=\frac{i}{\hbar}H_{bb}'e^Bc_b+e^B\dot c_b
\end{align*}

By equation (1) substitute for $\dot c_a$ and $\dot c_b$.
\begin{align*}
\dot d_a&=\frac{i}{\hbar}H_{aa}'e^Ac_a
-\frac{i}{\hbar}e^A\left(c_aH_{aa}'+c_bH_{ab}'e^{-i\omega_0t}\right)
\\
\dot d_b&=\frac{i}{\hbar}H_{bb}'e^Bc_b
-\frac{i}{\hbar}e^B\left(c_bH_{bb}'+c_aH_{ba}'e^{i\omega_0t}\right)
\end{align*}

Expand right-hand sides.
\begin{align*}
\dot d_a&=\frac{i}{\hbar}H_{aa}'e^Ac_a
-\frac{i}{\hbar}H_{aa}'e^Ac_a
-\frac{i}{\hbar}e^Ac_bH_{ab}'e^{-i\omega_0t}
\\
\dot d_b&=\frac{i}{\hbar}H_{bb}'e^Bc_b
-\frac{i}{\hbar}H_{bb}'e^Bc_b
-\frac{i}{\hbar}e^Bc_aH_{ba}'e^{i\omega_0t}
\end{align*}

Cancel terms.
\begin{align*}
\dot d_a&=-\frac{i}{\hbar}e^Ac_bH_{ab}'e^{-i\omega_0t}
\\
\dot d_b&=-\frac{i}{\hbar}e^Bc_aH_{ba}'e^{i\omega_0t}
\end{align*}

By equation (2) we have for $c_a$ and $c_b$
\begin{equation*}
c_a=e^{-A}d_a,\quad
c_b=e^{-B}d_b
\end{equation*}

Hence by substitution for $c_a$ and $c_b$
\begin{align*}
\dot d_a&=-\frac{i}{\hbar}e^Ae^{-B}H_{ab}'e^{-i\omega_0t}d_b
\\
\dot d_b&=-\frac{i}{\hbar}e^Be^{-A}H_{ba}'e^{i\omega_0t}d_a
\end{align*}

Let
\begin{equation*}
e^{i\phi}=e^Ae^{-B}=e^{A-B}
=\exp\left(\frac{i}{\hbar}\int_0^t\left[H_{aa}'(t')-H_{bb}'(t')\right]dt'\right)
\end{equation*}

Then
\begin{align*}
\dot d_a&=-\frac{i}{\hbar}e^{i\phi}H_{ab}'e^{-i\omega_0t}d_b
\\
\dot d_b&=-\frac{i}{\hbar}e^{-i\phi}H_{ba}'e^{i\omega_0t}d_a
\end{align*}

\end{document}
