\documentclass[12pt]{article}
\usepackage{amsmath}
\parindent=0pt
\begin{document}

Let $|\Psi\rangle$ be a coherent state where $\bar n$ is the expected number of photons.
\begin{equation*}
|\Psi\rangle=\sum_{n=0}^\infty
\sqrt{\frac{\bar n^n\exp(-\bar n)}{n!}}
\exp\left(-i\left(n+\tfrac{1}{2}\right)\omega t\right)
|n\rangle
\end{equation*}

Operator $\hat a$ is an eigenfunction of $|\Psi\rangle$.
\begin{align*}
\hat a|\Psi\rangle&=\sqrt{\bar n}\exp(-i\omega t)|\Psi\rangle
\\
\langle\Psi|\hat a^\dag&=\left(\hat a|\Psi\rangle\right)^\dag=\sqrt{\bar n}\exp(i\omega t)\langle\Psi|
\end{align*}

Let $\hat E$ be the electric field operator
\begin{equation*}
\hat E=i\sqrt{\frac{\hbar\omega}{2\epsilon_0}}
(\hat a-\hat a^\dag)
\end{equation*}

Note that $\hat E$ is Hermitian.
\begin{equation*}
\hat E=\hat E^\dag
\end{equation*}

The expected electric field is
\begin{equation*}
\langle\hat E\rangle
=\langle\Psi|\hat E|\Psi\rangle
=i\sqrt{\frac{\hbar\omega}{2\epsilon_0}}
\langle\Psi|(\hat a-\hat a^\dag)|\Psi\rangle
\end{equation*}

By distributive law
\begin{equation*}
\langle\hat E\rangle
=i\sqrt{\frac{\hbar\omega}{2\epsilon_0}}
\left(\langle\Psi|\hat a|\Psi\rangle-\langle\Psi|\hat a^\dag|\Psi\rangle\right)
\end{equation*}

Substitute eigenvalues for operators.
\begin{equation*}
\langle\hat E\rangle
=i\sqrt{\frac{\hbar\omega}{2\epsilon_0}}
\left(\sqrt{\bar n}\exp(-i\omega t)\langle\Psi|\Psi\rangle-\sqrt{\bar n}\exp(i\omega t)\langle\Psi|\Psi\rangle\right)
\end{equation*}

By $\langle\Psi|\Psi\rangle=1$ we have
\begin{equation*}
\langle\hat E\rangle
=i\sqrt{\frac{\hbar\omega}{2\epsilon_0}}
\left(\sqrt{\bar n}\exp(-i\omega t)-\sqrt{\bar n}\exp(i\omega t)\right)
\end{equation*}

Recalling that
\begin{equation*}
2\sin(\omega t)=i\exp(-i\omega t)-i\exp(i\omega t)
\end{equation*}
we have
\begin{equation*}
\langle\hat E\rangle=\sqrt{\frac{2\bar n\hbar\omega}{\epsilon_0}}\sin(\omega t)
\end{equation*}

Let $\hat B$ be the magnetic field operator
\begin{equation*}
\hat B=\sqrt{\frac{\hbar\omega\mu_0}{2}}
(\hat a+\hat a^\dag)
\end{equation*}

By deduction similar to that for $\langle\hat E\rangle$ we obtain
\begin{equation*}
\langle\hat B\rangle=\sqrt{2\bar n\hbar\omega\mu_0}\cos(\omega t)
\end{equation*}

The energy of an electromagnetic wave is
\begin{equation*}
U=\frac{\epsilon_0}{2}|\mathbf E|^2+\frac{1}{2\mu_0}|\mathbf B|^2
\end{equation*}

For linear polarization and a suitable rotation matrix $R$ we have
\begin{equation*}
R\mathbf E=\begin{pmatrix}E\\0\\0\end{pmatrix},
\quad
R\mathbf B=\begin{pmatrix}0\\B\\0\end{pmatrix}
\end{equation*}

Hence in the rotated frame
\begin{equation*}
U=\frac{\epsilon_0}{2}E^2+\frac{1}{2\mu_0}B^2
\end{equation*}

For a quantum field we have
\begin{equation*}
U=\frac{\epsilon_0}{2}\langle\hat E^2\rangle+\frac{1}{2\mu_0}\langle\hat B^2\rangle
\end{equation*}
where
\begin{align*}
\langle\hat E^2\rangle
&=\langle\Psi|\hat E\hat E|\Psi\rangle
=-\frac{\hbar\omega}{2\epsilon_0}
\langle\Psi|(\hat a-\hat a^\dag)(\hat a-\hat a^\dag)|\Psi\rangle
\\
\langle\hat B^2\rangle
&=\langle\Psi|\hat B\hat B|\Psi\rangle
=\frac{\hbar\omega\mu_0}{2}
\langle\Psi|(\hat a+\hat a^\dag)(\hat a+\hat a^\dag)|\Psi\rangle
\end{align*}

For the coherent state
\begin{align*}
\langle\Psi|\hat a\hat a|\Psi\rangle&=\left(\sqrt{\bar n}\exp(-i\omega t)\right)^2
& &=\bar n\exp(-2i\omega t)
\\
\langle\Psi|\hat a^\dag\hat a|\Psi\rangle
&=\left(\sqrt{\bar n}\exp(i\omega t)\right)\left(\sqrt{\bar n}\exp(-i\omega t)\right)
& &=\bar n
\\
\langle\Psi|\hat a\hat a^\dag|\Psi\rangle&=\langle\Psi|(\hat a^\dag\hat a+1)|\Psi\rangle
=\langle\Psi|a^\dag\hat a|\Psi\rangle+\langle\Psi|\Psi\rangle
& &=\bar n+1
\\
\langle\Psi|\hat a^\dag\hat a^\dag|\Psi\rangle&=\left(\sqrt{\bar n}\exp(i\omega t)\right)^2
& &=\bar n\exp(2i\omega t)
\end{align*}

The expectation $\bar n+1$ for $\hat a\hat a^\dag$ is from the commutator
\begin{equation*}
\hat a\hat a^\dag-\hat a^\dag\hat a=1
\end{equation*}

Using the expectation values derived above we now have
\begin{align*}
\langle\hat E^2\rangle
&=-\frac{\hbar\omega}{2\epsilon_0}
\left(\bar n\exp(-2i\omega t)+\bar n\exp(2i\omega t)-2\bar n-1\right)
\\
\langle\hat B^2\rangle
&=\frac{\hbar\omega\mu_0}{2}
\left(\bar n\exp(-2i\omega t)+\bar n\exp(2i\omega t)+2\bar n+1\right)
\end{align*}

Noting that
\begin{align*}
-4\sin(\omega t)^2&=\exp(-2i\omega t)+\exp(2i\omega t)-2\\
4\cos(\omega t)^2&=\exp(-2i\omega t)+\exp(2i\omega t)+2
\end{align*}
we have
\begin{align*}
\langle\hat E^2\rangle
&=-\frac{\hbar\omega}{2\epsilon_0}\left(-4\bar n\sin(\omega t)^2-1\right)
\\
\langle\hat B^2\rangle
&=\frac{\hbar\omega\mu_0}{2}\left(4\bar n\cos(\omega t)^2+1\right)
\end{align*}

Rewrite as
\begin{align*}
\frac{\epsilon_0}{2}\langle\hat E^2\rangle&=\hbar\omega\left(\bar n\sin(\omega t)^2+\tfrac{1}{4}\right)
\\
\frac{1}{2\mu_0}\langle\hat B^2\rangle&=\hbar\omega\left(\bar n\cos(\omega t)^2+\tfrac{1}{4}\right)
\end{align*}

Hence the total energy per unit volume is
\begin{equation*}
U=\frac{\epsilon_0}{2}\langle\hat E^2\rangle
+\frac{1}{2\mu_0}\langle\hat B^2\rangle
=\hbar\omega\left(\bar n+\tfrac{1}{2}\right)
\end{equation*}

Check units.
\begin{equation*}
\hbar\omega=h\nu\propto\text{joule}\,\text{second}\times\frac{1}{\text{second}}=\text{joule}
\end{equation*}

We will now show that
\begin{equation*}
\hat a|\Psi\rangle=\sqrt{\bar n}\exp(-i\omega t)|\Psi\rangle
\end{equation*}

Apply operator $\hat a$ to coherent state $|\Psi\rangle$ to obtain
\begin{equation*}
\hat a|\Psi\rangle
=\sum_{n=0}^\infty
\sqrt{\frac{\bar n^n\exp(-\bar n)}{n!}}
\exp\left(-i\left(n+\tfrac{1}{2}\right)\omega t\right)
\sqrt n|n-1\rangle
\end{equation*}

The $n=0$ term vanishes hence the sum can start from $n=1$.
\begin{equation*}
\hat a|\Psi\rangle
=\sum_{n=1}^\infty
\sqrt{\frac{\bar n^n\exp(-\bar n)}{n!}}
\exp\left(-i\left(n+\tfrac{1}{2}\right)\omega t\right)
\sqrt n|n-1\rangle
\end{equation*}

The $\sqrt n$ cancels with $n$ factorial.
\begin{equation*}
\hat a|\Psi\rangle
=\sum_{n=1}^\infty
\sqrt{\frac{\bar n^n\exp(-\bar n)}{(n-1)!}}
\exp\left(-i\left(n+\tfrac{1}{2}\right)\omega t\right)
|n-1\rangle
\end{equation*}

Factor out $\sqrt{\bar n}\exp(-i\omega t)$.
\begin{equation*}
\hat a|\Psi\rangle
=\sqrt{\bar n}\exp(-i\omega t)
\sum_{n=1}^\infty
\sqrt{\frac{\bar n^{n-1}\exp(-\bar n)}{(n-1)!}}
\exp\left(-i\left(n-\tfrac{1}{2}\right)\omega t\right)
|n-1\rangle
\end{equation*}

Substitute $n+1$ for index $n$.
\begin{equation*}
\hat a|\Psi\rangle
=\sqrt{\bar n}\exp(-i\omega t)
\sum_{n=0}^\infty
\sqrt{\frac{\bar n^n\exp(-\bar n)}{n!}}
\exp\left(-i\left(n+\tfrac{1}{2}\right)\omega t\right)
|n\rangle
\end{equation*}

Hence
\begin{equation*}
\hat a|\Psi\rangle=\sqrt{\bar n}\exp(-i\omega t)|\Psi\rangle
\end{equation*}

\section*{Energy states}
For state $|n\rangle$ we have
\begin{align*}
\langle n|\hat a\hat a|n\rangle&=0
\\
\langle n|\hat a\hat a^\dag|n\rangle&=n+1
\\
\langle n|\hat a^\dag\hat a|n\rangle&=n
\\
\langle n|\hat a^\dag\hat a^\dag|n\rangle&=0
\end{align*}

Hence
\begin{align*}
\langle\hat E^2\rangle
&=-\frac{\hbar\omega}{2\epsilon_0}(-2n-1)
\\
\langle\hat B^2\rangle
&=\frac{\hbar\omega\mu_0}{2}(2n+1)
\end{align*}

Rewrite as
\begin{align*}
\frac{\epsilon_0}{2}\langle\hat E^2\rangle&=\hbar\omega\left(\tfrac{1}{2}n+\tfrac{1}{4}\right)
\\
\frac{1}{2\mu_0}\langle\hat B^2\rangle&=\hbar\omega\left(\tfrac{1}{2}n+\tfrac{1}{4}\right)
\end{align*}

Hence the total energy per unit volume is
\begin{equation*}
U=\frac{\epsilon_0}{2}\langle\hat E^2\rangle
+\frac{1}{2\mu_0}\langle\hat B^2\rangle
=\hbar\omega\left(n+\tfrac{1}{2}\right)
\end{equation*}

\end{document}
