\documentclass[12pt]{article}
\usepackage{amsmath}
\usepackage{amssymb}

\parindent=0pt

\newcommand\INT{\int_{\mathbb R^3}}

\begin{document}

7-2.
If $F\big(x(t)\big)=x(t)$, show that
\begin{equation*}
\frac{\delta F}{\delta x(s)}=\delta(t-s)
\end{equation*}

\bigskip
\hrule

\bigskip
Consider equation (7.20).
\begin{equation*}
F\big(x(t)+\eta(t)\big)=F\big(x(t)\big)+\int\frac{\delta F}{\delta x(s)}\eta(s)\,ds+\cdots
\tag{7.20}
\end{equation*}

For $F\big(x(t)\big)=x(t)$ we have
\begin{equation*}
F\big(x(t)+\eta(t)\big)=x(t)+\eta(t)
\end{equation*}

Then by equation (7.20) to first order
\begin{equation*}
\eta(t)=\int\frac{\delta F}{\delta x(s)}\eta(s)\,ds
\end{equation*}

Hence
\begin{equation*}
\frac{\delta F}{\delta x(s)}=
\begin{cases}
1 & t=s
\\
0 & t\ne s
\end{cases}
\end{equation*}


\end{document}
