\documentclass[12pt]{article}
\usepackage{amsmath}
\usepackage{amssymb}

\parindent=0pt

\begin{document}

8-4.
Show that the ground-state wave function for the Lagrangian of
equation (8.78) can be written
\begin{equation*}
\Phi_0=A\exp\left(
-\frac{1}{2\hbar}
\sum_{\alpha=1}^{N-1}
\omega_\alpha Q_\alpha^*Q_\alpha
\right)
\tag{8.83}
\end{equation*}
(where $A$ is a constant) by starting with the wave function in terms of
the real variables $Q_\alpha^c$ and $Q_\alpha^s$.
\begin{gather*}
L=\frac{1}{2}\sum_{\alpha=0}^{N-1}
\left(\dot Q_\alpha^*\dot Q_\alpha-\omega_\alpha^2Q_\alpha^*Q_\alpha\right)
\tag{8.78}
\\
Q_\alpha^c=\frac{1}{\sqrt2}(Q_\alpha+Q_\alpha^*)
\tag{8.79}
\\
Q_\alpha^s=\frac{i}{\sqrt2}(Q_\alpha-Q_\alpha^*)
\tag{8.80}
\end{gather*}

Rewrite (8.78) as
\begin{equation*}
L=\frac{1}{2}\dot Q_0^*\dot Q_0
-\frac{1}{2}\omega_0^2Q_0^*Q_0
+\frac{1}{2}\sum_{\alpha=1}^{N-1}
\left(\dot Q_\alpha^*\dot Q_\alpha-\omega_\alpha^2Q_\alpha^*Q_\alpha\right)
\end{equation*}

Note that
\begin{align*}
Q_\alpha^*Q_\alpha
&=\frac{1}{2}(Q_\alpha^c+iQ_\alpha^s)(Q_\alpha^c-iQ_\alpha^s)
\\
&=\frac{1}{2}(Q_\alpha^c)^2+\frac{1}{2}(Q_\alpha^s)^2
\end{align*}
and
\begin{equation*}
Q_0^s=0
\end{equation*}

Hence
\begin{equation*}
L=\frac{1}{4}(\dot Q_0^c)^2-\frac{1}{4}\omega^2(Q_0^c)^2
+\frac{1}{4}\sum_{\alpha=1}^{N-1}
\left(
(\dot Q_\alpha^c)^2
+(\dot Q_\alpha^s)^2
-\omega_\alpha^2(Q_\alpha^c)^2
-\omega_\alpha^2(Q_\alpha^s)^2
\right)
\end{equation*}

% FIXME go from L to wave function

\end{document}
