\documentclass[12pt]{article}
\usepackage{amsmath}
\usepackage{amssymb}

\parindent=0pt

\newcommand\INT{\int_{\mathbb R^3}}

\begin{document}

4-4.
Show that
\begin{equation*}
\frac{\partial^2}{\partial x^2}x=x\frac{\partial^2}{\partial x^2}+2\frac{\partial}{\partial x}
\tag{4.22}
\end{equation*}
and therefore for the $H$ in equation (4.15)
\begin{equation*}
Hx-xH=-\frac{\hbar^2}{m}\frac{\partial}{\partial x}
\end{equation*}

\bigskip
\hrule

\bigskip
We have
\begin{equation*}
\frac{\partial}{\partial x}(x\psi)=\psi+x\frac{\partial}{\partial x}\psi
\end{equation*}

Differentiate a second time.
\begin{align*}
\frac{\partial^2}{\partial x^2}(x\psi)
&=\frac{\partial}{\partial x}\left(\psi+x\frac{\partial}{\partial x}\psi\right)
\\
&=\frac{\partial}{\partial x}\psi+\frac{\partial}{\partial x}\psi+x\frac{\partial^2}{\partial x^2}\psi
\\
&=2\frac{\partial}{\partial x}\psi+x\frac{\partial^2}{\partial x^2}\psi
\end{align*}

This is equation (4.15).
\begin{equation*}
H=-\frac{\hbar^2}{2m}\frac{\partial^2}{\partial x^2}+V(x,t)
\end{equation*}

Solve for $\partial^2/\partial x^2$.
\begin{equation*}
\frac{\partial^2}{\partial x^2}=-\frac{2m}{\hbar^2}(H-V(x,t))
\tag{1}
\end{equation*}

By equation (4.22) above
\begin{equation*}
\frac{\partial^2}{\partial x^2}x-x\frac{\partial^2}{\partial x^2}=2\frac{\partial}{\partial x}
\tag{2}
\end{equation*}

Substitute (1) into (2).
\begin{equation*}
-\frac{2m}{\hbar^2}(H-V(x,t))x+x\frac{2m}{\hbar^2}(H-V(x,t))=2\frac{\partial}{\partial x}
\end{equation*}

The two $V$ terms cancel.
Multiply both sides by $-\hbar^2/2m$.
\begin{equation*}
Hx-xH=-\frac{\hbar^2}{m}\frac{\partial}{\partial x}
\end{equation*}

\end{document}
