\documentclass[12pt]{article}
\usepackage{amsmath}

\parindent=0pt

\begin{document}

3-8.
This is the Lagrangian for a harmonic oscillator.
\begin{equation*}
L=\frac{m}{2}\dot x^2-\frac{m\omega^2}{2}x^2
\end{equation*}

Show that the resulting kernel is
\begin{equation*}
K=F(T)\exp\left(
\frac{im\omega}{2\hbar\sin(\omega T)}
\left((x_b^2+x_a^2)\cos(\omega T)-2x_b x_a\right)
\right)
\end{equation*}
where $T=t_b-t_a$.

\bigskip
From problem 2-2 we have
\begin{equation*}
S_{cl}=\frac{m\omega}{2\hbar\sin(\omega T)}
\left((x_b^2+x_a^2)\cos(\omega T)-2x_b x_a\right)
\end{equation*}

From equation (3.51)
\begin{equation*}
K=F(T)\exp\left(
\frac{iS_{cl}}{\hbar}
\right)
\end{equation*}

By substitution of $S_{cl}$
\begin{equation*}
K=F(T)\exp\left(
\frac{im\omega}{2\hbar\sin(\omega T)}
\left((x_b^2+x_a^2)\cos(\omega T)-2x_b x_a\right)
\right)
\end{equation*}

\end{document}
