\documentclass[12pt]{article}
\usepackage{amsmath}

\parindent=0pt

\begin{document}

2-1.
For a free particle $L=(m/2)\dot x^2.$
Show that the action $S_{cl}$ corresponding to the classical motion
of a free particle is
\begin{equation*}
S_{cl}=\frac{m}{2}\frac{(x_b-x_a)^2}{t_b-t_a}
\tag{2.8}
\end{equation*}

\bigskip
\hrule

\bigskip
We will need the following equations.
\begin{gather*}
S=\int_{t_a}^{t_b} L\,dt
\tag{2.1}
\\
\frac{d}{dt}\frac{\partial L}{\partial\dot x}=\frac{\partial L}{\partial x}
\tag{2.7}
\end{gather*}

For $L=(m/2)\dot x^2$ we have
\begin{equation*}
\frac{d}{dt}\frac{\partial L}{\partial\dot x}=m\ddot x
\qquad
\frac{\partial L}{\partial x}=0
\end{equation*}

By equation (2.7)
\begin{equation*}
\ddot x=0
\end{equation*}

Hence velocity $\dot x$ is constant and equals distance divided by time.
\begin{equation*}
\dot x=\frac{x_b-x_a}{t_b-t_a}
\tag{1}
\end{equation*}

Substitute (1) into the Lagrangian.
\begin{equation*}
L=\frac{m}{2}\left(\frac{x_b-x_a}{t_b-t_a}\right)^2
\tag{2}
\end{equation*}

Substitute (2) into (2.1) to obtain
\begin{equation*}
S_{cl}=\int_{t_a}^{t_b}\frac{m}{2}\left(\frac{x_b-x_a}{t_b-t_a}\right)^2\,dt
\tag{3}
\end{equation*}

Solve the integral in (3).
\begin{equation*}
S_{cl}
=\frac{m}{2}\left(\frac{x_b-x_a}{t_b-t_a}\right)^2 t\,\bigg|_{t_a}^{t_b}
=\frac{m}{2}\frac{(x_b-x_a)^2}{t_b-t_a}
\end{equation*}

\end{document}
