\documentclass[12pt]{article}
\usepackage{amsmath}

\parindent=0pt

\begin{document}

\begin{center}
Feynman and Hibbs problem 2-3
\end{center}

Find $S_{cl}$ for a particle under a constant force $f$, that is,
\begin{equation*}
L=\frac{m}{2}\dot x^2+fx
\end{equation*}

From the above Lagrangian we have
\begin{equation*}
\frac{d}{dt}\left(\frac{\partial L}{\partial\dot x}\right)=m\ddot x
\end{equation*}
and
\begin{equation*}
\frac{\partial L}{\partial x}=f
\end{equation*}

By equation (2.7) which is
\begin{equation*}
\frac{d}{dt}\left(\frac{\partial L}{\partial\dot x}\right)=\frac{\partial L}{\partial x}
\end{equation*}
we have
\begin{equation*}
\ddot x=\frac{f}{m}
\end{equation*}

Hence $x(t)$ must have the following quadratic form.
\begin{equation*}
x(t)=\frac{f}{2m}t^2+Bt+C
\end{equation*}

We have the following boundary conditions.
\begin{align*}
x(t_a)=x_a\\
x(t_b)=x_b
\end{align*}

Subtract to cancel $C$.
\begin{equation*}
x(t_b)-x(t_a)=\frac{f}{2m}\left(t_b^2-t_a^2\right)+B(t_b-t_a)=x_b-x_a
\end{equation*}

Solve for $B$.
\begin{equation*}
B=\frac{x_b-x_a}{t_b-t_a}-\frac{f\,\left(t_b^2-t_a^2\right)}{2m(t_b-t_a)}
\end{equation*}

Solve for C.
\begin{align*}
C&=x_a-\frac{f}{2m}t_a^2-Bt_a
\\[1ex]
&=\frac{f\,\left(t_a t_b^2 - t_a^2 t_b\right)}{2 m (t_b - t_a)} + \frac{t_b x_a - t_a x_b}{t_b - t_a}
\end{align*}

Altogether we have
\begin{equation*}
x(t)=
\frac{f}{2m}t^2
+\left(\frac{x_b-x_a}{t_b-t_a}-\frac{f\,\left(t_b^2-t_a^2\right)}{2m(t_b-t_a)}\right)t
+\frac{f\,\left(t_a t_b^2 - t_a^2 t_b\right)}{2 m (t_b - t_a)} + \frac{t_b x_a - t_a x_b}{t_b - t_a}
\tag{1}
\end{equation*}

Equation (1) is too complicated to continue so we now translate the time coordinate as
\begin{align*}
t_a=0
\\
t_b=T
\end{align*}
We now have
\begin{equation*}
x(t)=\frac{ft^2}{2m}+\left(\frac{x_b-x_a}{T}-\frac{fT}{2m}\right)t+x_a
\tag{2}
\end{equation*}

Differentiate $x(t)$ to obtain $\dot x(t)$.
\begin{equation*}
\dot x(t)=
\frac{d}{dt}x(t)=\frac{ft}{m}-\frac{fT}{2m}+\frac{x_b-x_a}{T}
\tag{3}
\end{equation*}

The new Lagrangian is
\begin{align*}
L&=\frac{m}{2}\dot x(t)^2+fx(t)
\\[1ex]
&=\frac{f^2}{m}t^2
+\left(\frac{2f\,(x_b-x_a)}{T}-\frac{f^2T}{m}\right)t
+\frac{f^2T^2}{8m}
+\frac{f\,(3x_a-x_b)}{2}
+\frac{m(x_b-x_a)^2}{2T^2}
\tag{4}
\end{align*}

Hence
\begin{equation*}
S_{cl}=\int_0^T L\,dt
=\frac{m(x_b-x_a)^2}{2T}+\frac{fT(x_b+x_a)}{2}-\frac{f^2T^3}{24m}
\tag{5}
\end{equation*}
where $T=t_b-t_a$.

\end{document}
