\documentclass[12pt]{article}
\usepackage{amsmath}

\parindent=0pt

\begin{document}

2-4.
Classically, the momentum is defined as
\begin{equation*}
p=\frac{\partial L}{\partial\dot x}
\tag{2.10}
\end{equation*}

Show that the momentum at a final point is
\begin{equation*}
\left(\frac{\partial L}{\partial\dot x}\right)_{x=x_b}
=+\frac{\partial S_{cl}}{\partial x_b}
\tag{2.11}
\end{equation*}
while the momentum at an initial point is
\begin{equation*}
\left(\frac{\partial L}{\partial\dot x}\right)_{x=x_a}
=-\frac{\partial S_{cl}}{\partial x_a}
\end{equation*}

{\it Hint:} Consider the effect on equation (2.6)
of a change in the end points.
\begin{equation*}
\delta S=\left(\delta x(t)\frac{\partial L}{\partial\dot x}\right)_{t_a}^{t_b}
-\int_{t_a}^{t_b}\delta x(t)
\left(\frac{d}{dt}\frac{\partial L}{\partial\dot x}
-\frac{\partial L}{\partial x}\right)\,dt
\tag{2.6}
\end{equation*}

\bigskip
\hrule

\bigskip
Consider equation (2.7) for the classical path.
\begin{equation*}
\frac{d}{dt}\frac{\partial L}{\partial\dot x}
-\frac{\partial L}{\partial x}=0
\tag{2.7}
\end{equation*}

Substitute (2.7) into (2.6) to obtain
\begin{equation*}
\delta S_{cl}=\left(\delta x(t)\frac{\partial L}{\partial\dot x}\right)_{t_a}^{t_b}
=\delta x_b\left(\frac{\partial L}{\partial\dot x}\right)_{x=x_b}
-\delta x_a\left(\frac{\partial L}{\partial\dot x}\right)_{x=x_a}
\tag{1}
\end{equation*}

For endpoints $a$ and $b$ we have $\delta S_{cl}=0$ by equation (2.3).
\begin{equation*}
\delta x_a=\delta x_b=0
\tag{2.3}
\end{equation*}

However, suppose endpoint $b$ is changed so that $\delta x_b\ne0$.
Then by (1)
\begin{equation*}
\delta S_{cl}=\delta x_b\left(\frac{\partial L}{\partial\dot x}\right)_{x=x_b}
\end{equation*}

It follows that
\begin{equation*}
\frac{\delta S_{cl}}{\delta x_b}
=\left(\frac{\partial L}{\partial\dot x}\right)_{x=x_b}
\end{equation*}
and in the limit
\begin{equation*}
\lim_{\delta\rightarrow0}\frac{\delta S_{cl}}{\delta x_b}=\frac{\partial S_{cl}}{\partial x_b}
=\left(\frac{\partial L}{\partial\dot x}\right)_{x=x_b}
\end{equation*}

Likewise, a change of endpoint $a$ yields
\begin{equation*}
\lim_{\delta\rightarrow0}\frac{\delta S_{cl}}{\delta x_a}=\frac{\partial S_{cl}}{\partial x_a}
=-\left(\frac{\partial L}{\partial\dot x}\right)_{x=x_a}
\end{equation*}

\end{document}
