\documentclass[12pt]{article}
\usepackage[margin=2cm]{geometry}
\usepackage{amsmath}

\begin{document}

\begin{align*}
r_1&=\sqrt{x_1^2+y_1^2+z_1^2}
\\
r_2&=\sqrt{x_2^2+y_2^2+z_2^2}
\\
r_{12}&=\sqrt{(x_1-x_2)^2+(y_1-y_2)^2+(z_1-z_2)^2}
\end{align*}

\noindent
The Halleraas coordinates are
\begin{align*}
s&=r_1+r_2
\\
t&=r_2-r_1
\\
u&=r_{12}
\end{align*}

\noindent
Hence
\begin{equation*}
\frac{\partial s}{\partial x_1}=\frac{x_1}{r_1}
\qquad
\frac{\partial t}{\partial x_1}=-\frac{x_1}{r_1}
\qquad
\frac{\partial u}{\partial x_1}=\frac{x_1-x_2}{r_{12}}
\end{equation*}

\begin{equation*}
\frac{\partial s}{\partial y_1}=\frac{y_1}{r_1}
\qquad
\frac{\partial t}{\partial y_1}=-\frac{y_1}{r_1}
\qquad
\frac{\partial u}{\partial y_1}=\frac{y_1-y_2}{r_{12}}
\end{equation*}

\begin{equation*}
\frac{\partial s}{\partial z_1}=\frac{z_1}{r_1}
\qquad
\frac{\partial t}{\partial z_1}=-\frac{z_1}{r_1}
\qquad
\frac{\partial u}{\partial z_1}=\frac{z_1-z_2}{r_{12}}
\end{equation*}

\noindent
Start by converting the Laplacian terms to Halleraas coordinates.
The first Laplacian is
\begin{equation*}
\nabla_1^2\psi
=\left(\frac{\partial\psi}{\partial x_1}\right)^2
+\left(\frac{\partial\psi}{\partial y_1}\right)^2
+\left(\frac{\partial\psi}{\partial z_1}\right)^2
\end{equation*}

\noindent
By the chain rule
\begin{equation*}
\frac{\partial\psi}{\partial x_1}
=\frac{\partial\psi}{\partial s}\frac{\partial s}{\partial x_1}
+\frac{\partial\psi}{\partial t}\frac{\partial t}{\partial x_1}
+\frac{\partial\psi}{\partial t}\frac{\partial t}{\partial x_1}
\end{equation*}

\noindent
Hence by (?)
\begin{equation*}
\frac{\partial\psi}{\partial x_1}
=\frac{x_1}{r_1}\frac{\partial\psi}{\partial s}
-\frac{x_1}{r_1}\frac{\partial\psi}{\partial t}
-\frac{x_2-x_1}{u}\frac{\partial\psi}{\partial u}
\end{equation*}

\noindent
And by symmetry for $y_1$ and $z_1$.
\begin{align*}
\frac{\partial\psi}{\partial y_1}
&=\frac{y_1}{r_1}\frac{\partial\psi}{\partial s}
-\frac{y_1}{r_1}\frac{\partial\psi}{\partial t}
-\frac{y_2-y_1}{u}\frac{\partial\psi}{\partial u}
\\
\frac{\partial\psi}{\partial z_1}
&=\frac{z_1}{r_1}\frac{\partial\psi}{\partial s}
-\frac{z_1}{r_1}\frac{\partial\psi}{\partial t}
-\frac{z_2-z_1}{u}\frac{\partial\psi}{\partial u}
\end{align*}

\noindent
Hence
\begin{equation*}
\nabla_1^2\psi
=\left(\frac{\partial\psi}{\partial s}\right)^2
+\left(\frac{\partial\psi}{\partial t}\right)^2
+\left(\frac{\partial\psi}{\partial u}\right)^2
-2\frac{\partial\psi}{\partial s}\frac{\partial\psi}{\partial t}
+2\left(\frac{\partial\psi}{\partial s}\frac{\partial\psi}{\partial u}
+\frac{\partial\psi}{\partial t}\frac{\partial\psi}{\partial u}\right)
\left(\text{more stuff here}\right)
\end{equation*}


\end{document}
