\documentclass[12pt]{article}
\usepackage[margin=2cm]{geometry}
\begin{document}

\noindent
$$
\left(\hat{H}_0+\epsilon\hat{V}\right)
\left(\psi_0+\epsilon\psi_1+\epsilon^2\psi_2\right)
=
\left(E_0+\epsilon E_1+\epsilon^2 E_2\right)
\left(\psi_0+\epsilon\psi_1+\epsilon^2\psi_2\right)
$$
Let $\epsilon=0$. Then
$$\hat{H}_0\psi_0=E_0\psi_0
$$
Let $\epsilon^1=1$ and $\epsilon^k=0$ for $k>1$. Then
$$
\hat{H}_0(\psi_0+\psi_1)+\hat{V}\psi_0
=
E_0(\psi_0+\psi_1)+E_1\psi_0
$$
Since $\hat{H}_0\psi_0=E_0\psi_0$ we can cancel $\hat{H}_0\psi_0$ with $E_0\psi_0$
and obtain
$$
\hat{H}_0\psi_1+\hat{V}\psi_0
=
E_0\psi_1+E_1\psi_0
$$
We want to solve for $E_1$.
Multiply both sides by $\psi_0^\dag$ and integrate over all space.
$$
\int_V\psi_0^\dag\left(\hat{H}_0\psi_1+\hat{V}\psi_0\right)\,dV
=
\int_V\psi_0^\dag\left(E_0\psi_1+E_1\psi_0\right)\,dV
$$
Then by the distributive property
$$
\int_V\psi_0^\dag\hat{H}_0\psi_1\,dV
+
\int_V\psi_0^\dag\hat{V}\psi_0\,dV
=
E_0\int_V\psi_0^\dag\psi_1\,dV
+
E_1\int_V\psi_0^\dag\psi_0\,dV
$$
Because $\hat{H}_0$ is Hermitian we have
$$
\psi_0^\dag\hat{H}_0\psi_1=(\hat{H}_0\psi_0)^\dag\psi_1=E_0\psi_0^\dag\psi_1
$$
Hence the $\hat{H}_0$ and $E_0$ integrals cancel.
We now have
$$
\int_V\psi_0^\dag\hat{V}\psi_0\,dV
=
E_1\int_V\psi_0^\dag\psi_0\,dV
$$
Rearrange to solve for $E_1$.
$$
E_1=\frac{\int_V\psi_0^\dag\hat{V}\psi_0\,dV}{\int_V\psi_0^\dag\psi_0\,dV}
$$

%\VerbatimInput[formatcom=\color{blue}]{polarized-light.txt}

\end{document}
