\documentclass[12pt]{article}
\usepackage{amsmath}
\parindent=0pt
\begin{document}

Exercise 6.4.
Use the matrix forms of $\sigma_z$, $\sigma_x$, and $\sigma_y$ and
the column vectors for $|u\}$ and $|d\}$ to verify Eqs.~6.6.
Then, use Eqs.~6.6 and 6.7 to write the equations that were left out
of Eqs.~6.8. Use the appendix to check your answers.

\bigskip
\hrule

\bigskip
\begin{equation*}
\sigma_z=\begin{pmatrix}1&0\\0&-1\end{pmatrix},
\quad
\sigma_x=\begin{pmatrix}0&1\\1&0\end{pmatrix},
\quad
\sigma_y=\begin{pmatrix}0&-i\\ i&0\end{pmatrix}
\tag{3.20}
\end{equation*}

\begin{equation*}
|u\}=\begin{pmatrix}1\\0\end{pmatrix},
\quad
|d\}=\begin{pmatrix}0\\1\end{pmatrix}
\end{equation*}

Hence
\begin{align*}
\sigma_z|u\}&=\begin{pmatrix}1&0\\0&-1\end{pmatrix}\begin{pmatrix}1\\0\end{pmatrix}=\begin{pmatrix}1\\0\end{pmatrix}=|u\}
\\[1ex]
\sigma_z|d\}&=\begin{pmatrix}1&0\\0&-1\end{pmatrix}\begin{pmatrix}0\\1\end{pmatrix}=\begin{pmatrix}0\\-1\end{pmatrix}=-|d\}
\\[1ex]
\sigma_x|u\}&=\begin{pmatrix}0&1\\1&0\end{pmatrix}\begin{pmatrix}1\\0\end{pmatrix}=\begin{pmatrix}0\\1\end{pmatrix}=|d\}
\\[1ex]
\sigma_x|d\}&=\begin{pmatrix}0&1\\1&0\end{pmatrix}\begin{pmatrix}0\\1\end{pmatrix}=\begin{pmatrix}1\\0\end{pmatrix}=|u\}
\\[1ex]
\sigma_y|u\}&=\begin{pmatrix}0&-i\\i&0\end{pmatrix}\begin{pmatrix}1\\0\end{pmatrix}=\begin{pmatrix}0\\i\end{pmatrix}=i|d\}
\\[1ex]
\sigma_y|d\}&=\begin{pmatrix}0&-i\\i&0\end{pmatrix}\begin{pmatrix}0\\1\end{pmatrix}=\begin{pmatrix}-i\\0\end{pmatrix}=-i|u\}
\end{align*}

The $\sigma$ operators operate on the left-hand side of the product state.

\bigskip
For $\sigma_z$ of product states we have
\begin{align*}
\sigma_z|uu\rangle&=\sigma_z|u\rangle\otimes|u\rangle
=|u\rangle\otimes|u\rangle=|uu\rangle
\\[1ex]
\sigma_z|ud\rangle&=\sigma_z|u\rangle\otimes|d\rangle
=|u\rangle\otimes|d\rangle=|ud\rangle
\\[1ex]
\sigma_z|du\rangle&=\sigma_z|d\rangle\otimes|u\rangle
=-|d\rangle\otimes|u\rangle=-|du\rangle
\\[1ex]
\sigma_z|dd\rangle&=\sigma_z|d\rangle\otimes|d\rangle
=-|d\rangle\otimes|d\rangle=-|dd\rangle
\end{align*}

For $\sigma_x$ of product states we have
\begin{align*}
\sigma_x|uu\rangle&=\sigma_x|u\rangle\otimes|u\rangle
=|d\rangle\otimes|u\rangle=|du\rangle
\\[1ex]
\sigma_x|ud\rangle&=\sigma_x|u\rangle\otimes|d\rangle
=|d\rangle\otimes|d\rangle=|dd\rangle
\\[1ex]
\sigma_x|du\rangle&=\sigma_x|d\rangle\otimes|u\rangle
=|u\rangle\otimes|u\rangle=|uu\rangle
\\[1ex]
\sigma_x|dd\rangle&=\sigma_x|d\rangle\otimes|d\rangle
=|u\rangle\otimes|d\rangle=|ud\rangle
\end{align*}

For $\sigma_y$ of product states we have
\begin{align*}
\sigma_y|uu\rangle&=\sigma_y|u\rangle\otimes|u\rangle
=i|d\rangle\otimes|u\rangle=i|du\rangle
\\[1ex]
\sigma_y|ud\rangle&=\sigma_y|u\rangle\otimes|d\rangle
=i|d\rangle\otimes|d\rangle=i|dd\rangle
\\[1ex]
\sigma_y|du\rangle&=\sigma_y|d\rangle\otimes|u\rangle
=-i|u\rangle\otimes|u\rangle=-i|uu\rangle
\\[1ex]
\sigma_y|dd\rangle&=\sigma_y|d\rangle\otimes|d\rangle
=-i|u\rangle\otimes|d\rangle=-i|ud\rangle
\end{align*}

The $\tau$ operators operate on the right-hand term of the product state.

\bigskip
For $\tau_z$ of product states we have
\begin{align*}
\tau_z|uu\rangle&=|u\rangle\otimes\tau_z|u\rangle
=|u\rangle\otimes|u\rangle=|uu\rangle
\\[1ex]
\tau_z|ud\rangle&=|u\rangle\otimes\tau_z|d\rangle
=|u\rangle\otimes-|d\rangle=-|ud\rangle
\\[1ex]
\tau_z|du\rangle&=|d\rangle\otimes\tau_z|u\rangle
=|d\rangle\otimes|u\rangle=|du\rangle
\\[1ex]
\tau_z|dd\rangle&=|d\rangle\otimes\tau_z|d\rangle
=|d\rangle\otimes-|d\rangle=-|dd\rangle
\end{align*}

For $\tau_x$ of product states we have
\begin{align*}
\tau_x|uu\rangle&=|u\rangle\otimes\tau_x|u\rangle
=|u\rangle\otimes|d\rangle=|ud\rangle
\\[1ex]
\tau_x|ud\rangle&=|u\rangle\otimes\tau_x|d\rangle
=|u\rangle\otimes|u\rangle=|uu\rangle
\\[1ex]
\tau_x|du\rangle&=|d\rangle\otimes\tau_x|u\rangle
=|d\rangle\otimes|d\rangle=|dd\rangle
\\[1ex]
\tau_x|dd\rangle&=|d\rangle\otimes\tau_x|d\rangle
=|d\rangle\otimes|u\rangle=|du\rangle
\end{align*}

For $\tau_y$ of product states we have
\begin{align*}
\tau_y|uu\rangle&=|u\rangle\otimes\tau_y|u\rangle
=|u\rangle\otimes i|d\rangle=i|ud\rangle
\\[1ex]
\tau_y|ud\rangle&=|u\rangle\otimes\tau_y|d\rangle
=|u\rangle\otimes-i|u\rangle=-i|uu\rangle
\\[1ex]
\tau_y|du\rangle&=|d\rangle\otimes\tau_y|u\rangle
=|d\rangle\otimes i|d\rangle=i|dd\rangle
\\[1ex]
\tau_y|dd\rangle&=|d\rangle\otimes\tau_y|d\rangle
=|d\rangle\otimes-i|u\rangle=-i|du\rangle
\end{align*}

\end{document}
