\documentclass[12pt]{article}
\usepackage{amsmath}
\parindent=0pt
\begin{document}

Exercise 4.2.
Prove that if $\mathbf M$ and $\mathbf L$ are both Hermitian,
$i[\mathbf M,\mathbf L]$ is also Hermitian.
Note that the $i$ is important.
The commutator is, by itself, not Hermitian.

\bigskip
\hrule

\bigskip
We have
\begin{equation*}
(i[\mathbf M,\mathbf L])^\dag=(i\mathbf M\mathbf L-i\mathbf L\mathbf M)^\dag
=-i(\mathbf M\mathbf L)^\dag+i(\mathbf L\mathbf M)^\dag
\end{equation*}

Noting that $(\mathbf M\mathbf L)^\dag=\mathbf L^\dag\mathbf M^\dag$ we have
\begin{equation*}
(i[\mathbf M,\mathbf L])^\dag
=-i\mathbf L^\dag\mathbf M^\dag+i\mathbf M^\dag\mathbf L^\dag
\end{equation*}

By hypothesis $\mathbf M=\mathbf M^\dag$ and $\mathbf L=\mathbf L^\dag$ hence
\begin{equation*}
(i[\mathbf M,\mathbf L])^\dag
=-i\mathbf L\mathbf M+i\mathbf M\mathbf L=i[\mathbf M,\mathbf L]
\end{equation*}

\end{document}
