\documentclass[12pt]{article}
\usepackage{amsmath}
\usepackage{amssymb}
\usepackage{mathrsfs} % \mathscr

\parindent=0pt

\begin{document}

5.12
Let $X_1$, $\ldots$, $X_n$ be a random sample from a $N(0,1)$
population. Define
$$Y_1=\left|{1\over n}\sum_{i=1}^n X_i\right|,\qquad
Y_2={1\over n}\sum_{i=1}^n|X_i|$$
Calculate $EY_1$ and $EY_2$, and establish an inequality between
them.

\bigskip
\noindent
For $Z\sim N(0,1)$ we have
\begin{eqnarray*}
E|Z|&=&2\cdot{1\over\sqrt{2\pi}}\int_0^\infty z\exp(-z^2/2)\,dz\\
&=&-\sqrt{2/\pi}\exp(-z^2/2)\bigg|_0^\infty\\
&=&\sqrt{2/\pi}
\end{eqnarray*}
By theorem 5.3.1 we have
$${1\over n}\sum_{i=1}^nX_i\sim N(0,1/n)$$
Noting that
$$Z/\sqrt n\sim N(0,1/n)$$
we have
$$EY_1=E|Z/\sqrt n|=E|Z|/\sqrt n=\sqrt{2/(n\pi)}$$
For $Y_2$ we have
$$EY_2={1\over n}\cdot nE|Z|=\sqrt{2/\pi}$$
Therefore
$$EY_1\le EY_2$$

\end{document}
