\input{preamble}

\section*{Angular momentum}

Definitions.
\begin{gather*}
\mathbf L=\mathbf X\times\mathbf P
=\begin{pmatrix}
X_2P_3-X_3P_2
\\
X_3P_1-X_1P_3
\\
X_1P_2-X_2P_1
\end{pmatrix}
\\[1ex]
L^2=|\mathbf L|^2=L_1^2+L_2^2+L_3^2
\\[1ex]
\mathbf J=\frac{1}{\hbar}\mathbf L
\end{gather*}

Show that

\begin{enumerate}

\item
\begin{equation*}
[\mathbf X,L_3]
=\begin{pmatrix}
-i\hbar X_2
\\
i\hbar X_1
\\
0
\end{pmatrix}
\end{equation*}

\item
\begin{equation*}
[\mathbf P,L_3]
=\begin{pmatrix}
-i\hbar P_2
\\
i\hbar P_1
\\
0
\end{pmatrix}
\end{equation*}

\item
\begin{equation*}
[\mathbf L,L^2]=0
\end{equation*}

\item
\begin{equation*}
\mathbf J\times\mathbf J=i\mathbf J
\end{equation*}

\item
\begin{equation*}
\mathbf P\times\mathbf L+\mathbf L\times\mathbf P=2i\hbar\mathbf P
\end{equation*}

\item
\begin{equation*}
\tfrac{1}{2}\left(\mathbf P\times\mathbf L-\mathbf L\times\mathbf P\right)
=\mathbf P\times\mathbf L-i\hbar\mathbf P
\end{equation*}

\item
\begin{equation*}
[L_i,P_j]=i\hbar\sum_k\epsilon_{ijk}P_k
\end{equation*}

\end{enumerate}

\end{document}
