\input{preamble}

\section*{Angular momentum 3}

The cross product in $\mathbf L=\mathbf r\times\mathbf p$ demands rectangular coordinates.
Hence for $\psi$ in spherical coordinates the vectors $\mathbf r$ and $\mathbf p$
must be transformed in $\mathbf L\psi$.

\bigskip
Vector $\mathbf r$ transforms as
\begin{equation*}
\mathbf r=\begin{pmatrix}x\\y\\z\end{pmatrix}
=\begin{pmatrix}
r\sin\theta\cos\phi
\\
r\sin\theta\sin\phi
\\
r\cos\theta
\end{pmatrix}
\end{equation*}

To transform $\mathbf p$ we have by the chain rule
\begin{align*}
\frac{\partial}{\partial x}
&=\sin\theta\cos\phi\frac{\partial}{\partial r}
+\frac{\cos\theta\cos\phi}{r}\frac{\partial}{\partial\theta}
-\frac{\sin\phi}{r\sin\theta}\frac{\partial}{\partial\phi}
\\[1ex]
\frac{\partial}{\partial y}
&=\sin\theta\sin\phi\frac{\partial}{\partial r}
+\frac{\cos\theta\sin\phi}{r}\frac{\partial}{\partial\theta}
+\frac{\cos\phi}{r\sin\theta}\frac{\partial}{\partial\phi}
\\[1ex]
\frac{\partial}{\partial z}
&=\cos\theta\frac{\partial}{\partial r}
-\frac{\sin\theta}{r}\frac{\partial}{\partial\theta}
\end{align*}

Hence
\begin{align*}
p_x&=-i\hbar\frac{\partial}{\partial x}=-i\hbar\left(
\sin\theta\cos\phi\frac{\partial}{\partial r}
+\frac{\cos\theta\cos\phi}{r}\frac{\partial}{\partial\theta}
-\frac{\sin\phi}{r\sin\theta}\frac{\partial}{\partial\phi}
\right)
\\[1ex]
p_y&=-i\hbar\frac{\partial}{\partial y}=-i\hbar\left(
\sin\theta\sin\phi\frac{\partial}{\partial r}
+\frac{\cos\theta\sin\phi}{r}\frac{\partial}{\partial\theta}
+\frac{\cos\phi}{r\sin\theta}\frac{\partial}{\partial\phi}
\right)
\\[1ex]
p_z&=-i\hbar\frac{\partial}{\partial z}=-i\hbar\left(
\cos\theta\frac{\partial}{\partial r}
-\frac{\sin\theta}{r}\frac{\partial}{\partial\theta}
\right)
\end{align*}

Using the transformed coordinates
\begin{align*}
x&=r\sin\theta\cos\phi
\\
y&=r\sin\theta\sin\phi
\\
z&=r\cos\theta
\end{align*}

we have for the angular momentum operators
\begin{align*}
L_x&=yp_z-zp_y=i\hbar\left(\sin\phi\frac{\partial}{\partial\theta}
+\frac{\cos\theta\cos\phi}{\sin\theta}\frac{\partial}{\partial\phi}\right)
\\[1ex]
L_y&=zp_x-xp_z=i\hbar\left(-\cos\phi\frac{\partial}{\partial\theta}
+\frac{\cos\theta\sin\phi}{\sin\theta}\frac{\partial}{\partial\phi}\right)
\\[1ex]
L_z&=xp_y-yp_x=-i\hbar\frac{\partial}{\partial\phi}
\end{align*}

and
\begin{equation*}
L^2={L_x}^2+{L_y}^2+{L_z}^2=-\hbar^2\left(
\frac{\cos\theta}{\sin\theta}\frac{\partial}{\partial\theta}
+\frac{\partial^2}{\partial\theta^2}+\frac{1}{\sin^2\theta}\frac{\partial^2}{\partial\phi^2}
\right)
\end{equation*}

\href{https://georgeweigt.github.io/examples/angular-momentum-3-demo.html}{Eigenmath script}

\end{document}
