\input{preamble}

\section*{Barrier potential}

Let $V(x)$ be the following barrier potential.
\begin{equation*}
V(x)=\begin{cases}
0 & x<-a
\\
V_0 & -a\le x\le a
\\
0 & x>a
\end{cases}
\end{equation*}

Find the transmission coefficient for this barrier potential.

\bigskip
Start with Schrodinger equations, one for each region of $V(x)$.
\begin{align*}
-\frac{\hbar^2}{2m}\frac{d^2}{dx^2}&\psi_1=E\psi_1, & x&\le-a
\\[1ex]
-\frac{\hbar^2}{2m}\frac{d^2}{dx^2}&\psi_2+V_0\psi_2=E\psi_2, & -a&\le x\le a
\\[1ex]
-\frac{\hbar^2}{2m}\frac{d^2}{dx^2}&\psi_3=E\psi_3, & x&\ge a
\end{align*}

The solutions are
\begin{align*}
\psi_1(x)&=A\exp(ikx)+B\exp(-ikx)
\\
\psi_2(x)&=C\exp(i\kappa x)+D\exp(-i\kappa x)
\\
\psi_3(x)&=F\exp(ikx)
\end{align*}

where
\begin{equation*}
k=\frac{\sqrt{2mE}}{\hbar},\quad
\kappa=\frac{\sqrt{2m(E-V_0)}}{\hbar}
\end{equation*}

Boundary conditions for $\psi_1$ and $\psi_2$.
\begin{equation*}
\psi_1(-a)=\psi_2(-a),\quad
\left.\frac{d\psi_1}{dx}\right|_{x=-a}=\left.\frac{d\psi_2}{dx}\right|_{x=-a}
\end{equation*}

Boundary conditions for $\psi_2$ and $\psi_3$.
\begin{equation*}
\psi_2(a)=\psi_3(a),\quad
\left.\frac{d\psi_2}{dx}\right|_{x=a}=\left.\frac{d\psi_3}{dx}\right|_{x=a}
\end{equation*}

From boundary conditions for $\psi_2$ and $\psi_3$ we have
\begin{equation*}
C\exp(i\kappa a)+D\exp(-i\kappa a)=F\exp(ikx)\tag{1}
\end{equation*}

and
\begin{equation*}
i\kappa C\exp(i\kappa a)-i\kappa D\exp(-i\kappa a)=ikF\exp(ikx)\tag{2}
\end{equation*}

Add $i\kappa$ times (1) to (2) to obtain
\begin{equation*}
2i\kappa C\exp(i\kappa a)=(i\kappa+ik)F\exp(ika)
\end{equation*}

Hence
\begin{equation*}
C=\frac{(\kappa+k)F\exp(ika-i\kappa a)}{2\kappa}
\end{equation*}

Add minus $i\kappa$ times (1) to (2) to obtain
\begin{equation*}
-2i\kappa D\exp(-i\kappa a)=(-i\kappa+ik)F\exp(ika)
\end{equation*}

Hence
\begin{equation*}
D=\frac{(\kappa-k)F\exp(ika+i\kappa a)}{2\kappa}
\end{equation*}

From boundary conditions for $\psi_1$ and $\psi_2$ we have
\begin{equation*}
A\exp(-ika)+B\exp(ika)=C\exp(-i\kappa a)+D\exp(i\kappa a)\tag{3}
\end{equation*}

and
\begin{equation*}
ikA\exp(-ika)-ikB\exp(ika)=i\kappa C\exp(-i\kappa a)-i\kappa D\exp(i\kappa a)\tag{4}
\end{equation*}

Add $ik$ times (3) to (4) to obtain
\begin{equation*}
2ikA\exp(-ika)=(ik+i\kappa)C\exp(-i\kappa a)+(ik-i\kappa)D\exp(i\kappa a)
\end{equation*}

Hence
\begin{equation*}
A=\frac{(k+\kappa)C\exp(ika-i\kappa a)}{2k}+\frac{(k-\kappa)D\exp(ika+i\kappa a)}{2k}
\end{equation*}

Add minus $ik$ times (3) to (4) to obtain
\begin{equation*}
-2ikB\exp(ika)=(-ik+i\kappa)C\exp(-i\kappa a)+(-ik-i\kappa)D\exp(i\kappa a)
\end{equation*}

Hence
\begin{equation*}
B=\frac{(k-\kappa)C\exp(-ika-i\kappa a)}{2k}+\frac{(k+\kappa)D\exp(-ika+i\kappa a)}{2k}
\end{equation*}

For transmission coefficient $T$ we have
\begin{equation*}
T^{-1}=\frac{A}{F}\left(\frac{A}{F}\right)^*
=1+\frac{1}{8}\left(\frac{E}{V_0-E}+\frac{V_0}{E}+1\right)
\left[\cos\left(\frac{4a}{\hbar}\sqrt{2m(E-V_0)}\right)-1\right]
\tag{5}
\end{equation*}

Equivalently
\begin{equation*}
T^{-1}=1+\frac{1}{4}\left(\frac{E}{V_0-E}+\frac{V_0}{E}+1\right)
\sinh^2\left(\frac{2ia}{\hbar}\sqrt{2m(E-V_0)}\right)
\tag{6}
\end{equation*}

Cancel the imaginary unit.
\begin{equation*}
T^{-1}=1+\frac{1}{4}\left(\frac{E}{V_0-E}+\frac{V_0}{E}+1\right)
\sinh^2\left(\frac{2a}{\hbar}\sqrt{2m(V_0-E)}\right)
\end{equation*}

Note that
\begin{equation*}
\frac{E}{V_0-E}+\frac{V_0}{E}+1=\frac{V_0^2}{E(V_0-E)}
\tag{7}
\end{equation*}

\end{document}
