\input{preamble}

\section*{Bhabha scattering}

Bhabha scattering is the process $e^-+e^+\rightarrow e^-+e^+$.

\begin{center}
\begin{tikzpicture}
\draw[dashed] (0,0) circle (0.5cm);
\draw[thick,->] (2,0) node[anchor=west] {$e^-$} -- (0.6,0);
\draw[thick,->] (-2,0) node[anchor=east] {$e^+$} -- (-0.6,0);
\draw[thick,->] (0.40,0.40) -- (1.3,1.3) node[anchor=south west] {$e^+$};
\draw[thick,->] (-0.4,-0.4) -- (-1.3,-1.3) node[anchor=north east] {$e^-$};
\draw (1,0.5) node {$\theta$};
\end{tikzpicture}
\end{center}

The following center-of-mass momentum vectors have $E=\sqrt{p^2+m^2}$.
\begin{equation*}
p_1=\underset{e^+ \, \longrightarrow}
{\begin{pmatrix}E\\0\\0\\p\end{pmatrix}}
\qquad
p_2=\underset{\longleftarrow \, e^-}
{\begin{pmatrix}E\\0\\0\\-p\end{pmatrix}}
\qquad
p_3=\underset{\substack{\phantom{e^+} \, \nearrow\\e^+ \, \phantom{\nearrow}}}
{\begin{pmatrix}E\\p\sin\theta\cos\phi\\p\sin\theta\sin\phi\\p\cos\theta\end{pmatrix}}
\qquad
p_4=\underset{\substack{\phantom{\swarrow} \, e^-\\\swarrow \, \phantom{e^-}}}
{\begin{pmatrix}E\\-p\sin\theta\cos\phi\\-p\sin\theta\sin\phi\\-p\cos\theta\end{pmatrix}}
\end{equation*}

Spinors for $p_1$.
\begin{equation*}
v_{11}=\frac{1}{\sqrt{E+m}}
\underset{\text{spin up}}
{\begin{pmatrix}p\\0\\E+m\\0\end{pmatrix}}
\qquad
v_{12}=\frac{1}{\sqrt{E+m}}
\underset{\text{spin down}}
{\begin{pmatrix}0\\-p\\0\\E+m\end{pmatrix}}
\end{equation*}

Spinors for $p_2$.
\begin{equation*}
u_{21}=\frac{1}{\sqrt{E+m}}
\underset{\text{spin up}}
{\begin{pmatrix}E+m\\0\\-p\\0\end{pmatrix}}
\qquad
u_{22}=\frac{1}{\sqrt{E+m}}
\underset{\text{spin down}}
{\begin{pmatrix}0\\E+m\\0\\p\end{pmatrix}}
\end{equation*}

Spinors for $p_3$.
\begin{equation*}
v_{31}=\frac{1}{\sqrt{E+m}}
\underset{\text{spin up}}
{\begin{pmatrix}p_{3z}\\p_{3x}+ip_{3y}\\E+m\\0\end{pmatrix}}
\qquad
v_{32}=\frac{1}{\sqrt{E+m}}
\underset{\text{spin down}}
{\begin{pmatrix}p_{3x}-ip_{3y}\\-p_{3z}\\0\\E+m\end{pmatrix}}
\end{equation*}

Spinors for $p_4$.
\begin{equation*}
u_{41}=\frac{1}{\sqrt{E+m}}
\underset{\text{spin up}}
{\begin{pmatrix}E+m\\0\\p_{4z}\\p_{4x}+ip_{4y}\end{pmatrix}}
\qquad
u_{42}=\frac{1}{\sqrt{E+m}}
\underset{\text{spin down}}
{\begin{pmatrix}0\\E+m\\p_{4x}-ip_{4y}\\-p_{4z}\end{pmatrix}}
\end{equation*}

The scattering amplitude $\mathcal M_{abcd}$ for spin state $abcd$ is
\begin{equation*}
\mathcal M_{abcd}=\mathcal M_{1abcd}+\mathcal M_{2abcd}
\end{equation*}

where
\begin{equation*}
\mathcal M_{1abcd}=-\frac{e^2}{t}
\underset{\text{scattering}}
{(\bar v_{1a}\gamma^\nu v_{3c})(\bar u_{4d}\gamma_\nu u_{2b})},
\quad
\mathcal M_{2abcd}=\frac{e^2}{s}
\underset{\text{annihilation}}
{(\bar v_{1a}\gamma^\mu u_{2b})(\bar u_{4d}\gamma_\mu v_{3c})}
\end{equation*}

Symbols $s$ and $t$ are Mandelstam variables.
\begin{align*}
s&=(p_1+p_2)^2
\\
t&=(p_1-p_3)^2
\end{align*}

Expected probability density $\langle|\mathcal M|^2\rangle$
is the sum of squared amplitudes divided by the number of inbound states.
\begin{equation*}
\langle|\mathcal M|^2\rangle=\frac{1}{4}\sum_{abcd}|\mathcal M_{abcd}|^2
\end{equation*}

Expand the summand and label the terms.
By positivity $\boxed{\scriptstyle2}=\boxed{\scriptstyle3}$.
\begin{equation*}
\langle|\mathcal{M}|^2\rangle=\frac{1}{4}
\sum_{abcd}
\bigl(
\underset{\boxed{\scriptstyle1}}{\mathcal M_{1abcd}\mathcal M_{1abcd}^*}+
\underset{\boxed{\scriptstyle2}}{\mathcal M_{1abcd}\mathcal M_{2abcd}^*}+
\underset{\boxed{\scriptstyle3}}{\mathcal M_{2abcd}\mathcal M_{1abcd}^*}+
\underset{\boxed{\scriptstyle4}}{\mathcal M_{2abcd}\mathcal M_{2abcd}^*}
\bigr)
\end{equation*}

The following Casimir trick uses matrix arithmetic to sum over spin states.
\begin{align*}
\sum_{abcd}{\boxed{\scriptstyle1}}
&=\frac{e^4}{t^2}\operatorname{Tr}\left[
(\slashed p_1-m)\gamma^\mu(\slashed p_3-m)\gamma^\nu
\right]
\operatorname{Tr}\left[
(\slashed p_4+m)\gamma_\mu(\slashed p_2+m)\gamma_\nu
\right]
\\
\sum_{abcd}{\boxed{\scriptstyle2}}
&=-\frac{e^4}{st}\operatorname{Tr}\left[
(\slashed p_1-m)\gamma^\mu(\slashed p_2+m)\gamma^\nu
(\slashed p_4+m)\gamma_\mu(\slashed p_3-m)\gamma_\nu
\right]
\\
\sum_{abcd}{\boxed{\scriptstyle4}}
&=\frac{e^4}{s^2}\operatorname{Tr}\left[
(\slashed p_1-m)\gamma^\mu(\slashed p_2+m)\gamma^\nu
\right]
\operatorname{Tr}\left[
(\slashed p_4+m)\gamma_\mu(\slashed p_3-m)\gamma_\nu
\right]
\end{align*}

Let
\begin{align*}
f_{11}&=\operatorname{Tr}\left[
(\slashed p_1-m)\gamma^\mu(\slashed p_3-m)\gamma^\nu
\right]
\operatorname{Tr}\left[
(\slashed p_4+m)\gamma_\mu(\slashed p_2+m)\gamma_\nu
\right]
\\
f_{12}&=-\operatorname{Tr}\left[
(\slashed p_1-m)\gamma^\mu(\slashed p_2+m)\gamma^\nu
(\slashed p_4+m)\gamma_\mu(\slashed p_3-m)\gamma_\nu
\right]
\\
f_{22}&=\operatorname{Tr}\left[
(\slashed p_1-m)\gamma^\mu(\slashed p_2+m)\gamma^\nu
\right]
\operatorname{Tr}\left[
(\slashed p_4+m)\gamma_\mu(\slashed p_3-m)\gamma_\nu
\right]
\end{align*}

so that
\begin{equation*}
\langle|\mathcal{M}|^2\rangle
=\frac{e^4}{4}
\left(
\frac{f_{11}}{t^2}+\frac{2f_{12}}{st}+\frac{f_{22}}{s^2}
\right)
\end{equation*}

The following formulas are equivalent to the Casimir trick.
(Recall that $a\cdot b=a^\mu g_{\mu\nu}b^\nu$)
\begin{align*}
f_{11}&=32 (p_1\cdot p_2)^2 + 32 (p_1\cdot p_4)^2 - 64 (p_1\cdot p_2) m^2 + 64 (p_1\cdot p_4) m^2
\\
f_{12}&=32 (p_1\cdot p_4)^2 + 64 (p_1\cdot p_4) m^2
\\
f_{22}&=32 (p_1\cdot p_3)^2 + 32 (p_1\cdot p_4)^2 + 64 (p_1\cdot p_3) m^2 + 64 (p_1\cdot p_4) m^2
\end{align*}

In Mandelstam variables
\begin{align*}
f_{11} &= 8 u^2 + 8 s^2 - 64 u m^2 - 64 s m^2 + 192 m^4
\\
f_{12} &= 8 u^2 - 64 u m^2 + 96 m^4
\\
f_{22} &= 8 u^2 + 8 t^2 - 64 u m^2 - 64 t m^2 + 192 m^4
\end{align*}

For $E\gg m$ a useful approximation is to set $m=0$ and obtain
\begin{align*}
f_{11}&=8u^2+8s^2
\\
f_{12}&=8u^2
\\
f_{22}&=8u^2+8t^2
\end{align*}

For $m=0$ the Mandelstam variables are
\begin{align*}
s&=4E^2
\\
t&=-2E^2(1-\cos\theta)
\\
u&=-2E^2(1+\cos\theta)
\end{align*}

Hence
\begin{align*}
\langle|\mathcal{M}|^2\rangle
&=\frac{e^4}{4}
\left(\frac{f_{11}}{t^2}+\frac{2f_{12}}{st}+\frac{f_{22}}{s^2}\right)
\\
&=2e^4\left(\frac{u^2+s^2}{t^2}+\frac{2u^2}{st}+\frac{u^2+t^2}{s^2}\right)
\\
&=e^4\biggl(
\underset{\text{scattering}}
{\frac{2(1+\cos\theta)^2+8}{(1-\cos\theta)^2}}
-\underset{\text{interaction}}
{\frac{2(1+\cos\theta)^2}{1-\cos\theta}}
+\underset{\text{annihilation}}
{1+\cos^2\theta}
\biggr)
\end{align*}

The expected probability density can be written more compactly as
\begin{equation*}
\langle|\mathcal{M}|^2\rangle=e^4\left(\frac{\cos^2\theta+3}{\cos\theta-1}\right)^2
\end{equation*}

\subsubsection*{Cross section}

The differential cross section is
\begin{equation*}
\frac{d\sigma}{d\Omega}=\frac{\langle|\mathcal{M}|^2\rangle}{4(4\pi\varepsilon_0)^2s}
\end{equation*}

where
\begin{equation*}
s=(p_1+p_2)^2=4E^2
\end{equation*}

For high energy experiments we have
\begin{equation*}
\langle|\mathcal{M}|^2\rangle=e^4\left(\frac{\cos^2\theta+3}{\cos\theta-1}\right)^2
\end{equation*}

Hence
\begin{equation*}
\frac{d\sigma}{d\Omega}=\frac{e^4}{4(4\pi\varepsilon_0)^2s}
\left(\frac{\cos^2\theta+3}{\cos\theta-1}\right)^2
\end{equation*}

Noting that
\begin{equation*}
e^2=4\pi\varepsilon_0\alpha\hbar c
\end{equation*}

we have
\begin{equation*}
\frac{d\sigma}{d\Omega}
=\frac{\alpha^2(\hbar c)^2}{4s}
\left(\frac{\cos^2\theta+3}{\cos\theta-1}\right)^2
\end{equation*}

Noting that
\begin{equation*}
d\Omega=\sin\theta\,d\theta\,d\phi
\end{equation*}

we also have
\begin{equation*}
d\sigma=\frac{\alpha^2(\hbar c)^2}{4s}
\left(\frac{\cos^2\theta+3}{\cos\theta-1}\right)^2
\sin\theta\,d\theta\,d\phi
\end{equation*}

Let $S(\theta_1,\theta_2)$ be the following integral of $d\sigma$.
\begin{equation*}
S(\theta_1,\theta_2)=\int_0^{2\pi}\int_{\theta_1}^{\theta_2}d\sigma
\end{equation*}

The solution is
\begin{equation*}
S(\theta_1,\theta_2)=\frac{\pi\alpha^2(\hbar c)^2}{2s}[I(\theta_2)-I(\theta_1)]
\end{equation*}

where
\begin{equation*}
I(\theta)=\frac{16}{\cos\theta-1}-\frac{\cos^3\theta}{3}-\cos^2\theta-9\cos\theta-16\log(1-\cos\theta)
\end{equation*}

The cumulative distribution function is
\begin{equation*}
F(\theta)
=\frac{S(a,\theta)}{S(a,\pi)}
=\frac{I(\theta)-I(a)}{I(\pi)-I(a)},
\quad
a\le\theta\le\pi
\end{equation*}

Angular support is reduced by an arbitrary angle $a>0$ because $I(0)$ is undefined.

\bigskip
The probability of observing scattering events in the interval $\theta_1$ to $\theta_2$ is
\begin{equation*}
P(\theta_1<\theta\le\theta_2)=F(\theta_2)-F(\theta_1)
\end{equation*}

The probability density function is
\begin{equation*}
f(\theta)=\frac{dF(\theta)}{d\theta}
=\frac{1}{I(\pi)-I(a)}
\left(\frac{\cos^2\theta+3}{\cos\theta-1}\right)^2
\sin\theta
\end{equation*}

\end{document}
