\input{preamble}

% Feynman and Hibbs problem 2-3

\section*{Constant force action}

This is the Lagrangian for a particle in a region of constant force $F$.
\begin{equation*}
L=\frac{m\dot x^2}{2}+Fx
\end{equation*}

Show that
\begin{equation*}
S=\int_0^TL\,dt=\frac{m(x_b-x_a)^2}{2T}+\frac{FT(x_b+x_a)}{2}-\frac{F^2T^3}{24m},\quad T=t_b-t_a
\end{equation*}

The first step is to derive $x(t)$ and $\dot x(t)$ from $L$ and the Euler-Lagrange equation
\begin{equation*}
\frac{d}{dt}\frac{\partial L}{\partial\dot x}=\frac{\partial L}{\partial x}
\end{equation*}

From $L$ we have
\begin{equation*}
\frac{d}{dt}\frac{\partial L}{\partial\dot x}=m\ddot x,\quad
\frac{\partial L}{\partial x}=F
\end{equation*}

and by Euler-Lagrange
\begin{equation*}
\ddot x=\frac{F}{m}
\end{equation*}

Note that
\begin{equation*}
\frac{d^2}{dt^2}\left(\frac{Ft^2}{2m}+At+B\right)=\frac{F}{m}=\ddot x
\end{equation*}

Hence $x(t)$ is quadratic.
\begin{equation*}
x(t)=\frac{Ft^2}{2m}+At+B
\end{equation*}

These are the boundary conditions.
\begin{equation*}
x(0)=x_a,\quad x(T)=x_b
\end{equation*}

Solve for $B$.
\begin{equation*}
x(0)=B=x_a
\end{equation*}

Solve for $A$.
\begin{equation*}
x(T)-x(0)=\frac{FT^2}{2m}+AT=x_b-x_a
\end{equation*}

Hence
\begin{equation*}
A=\frac{x_b-x_a}{T}-\frac{FT}{2m}
\end{equation*}

Substitute $A$ and $B$ into $x(t)$.
\begin{equation*}
x(t)=\frac{Ft^2}{2m}+\frac{(x_b-x_a)t}{T}-\frac{FTt}{2m}+x_a
\tag{1}
\end{equation*}

Take the time derivative of $x(t)$ to obtain $\dot x(t)$.
\begin{equation*}
\dot x(t)=\frac{d}{dt}x(t)=\frac{Ft}{m}+\frac{x_b-x_a}{T}-\frac{FT}{2m}
\tag{2}
\end{equation*}

The action is
\begin{align*}
S&=\int_0^TL\,dt
\\
&=\int_0^T\left(\frac{m\dot x^2}{2}+Fx\right)\,dt
\\
&=\frac{m(x_b-x_a)^2}{2T}+\frac{FT(x_b+x_a)}{2}-\frac{F^2T^3}{24m}
\tag{3}
\end{align*}

\end{document}
