\input{preamble}

\section*{Free particle action}

This is the Lagrangian for a free particle.
\begin{equation*}
L=\frac{m\dot x^2}{2}
\end{equation*}

Show that
\begin{equation*}
S=\int_0^TL\,dt=\frac{m(x_b-x_a)^2}{2T},\quad T=t_b-t_a
\end{equation*}

The first step is to derive $\dot x(t)$ from $L$ and the Euler-Lagrange equation
\begin{equation*}
\frac{d}{dt}\frac{\partial L}{\partial\dot x}=\frac{\partial L}{\partial x}
\end{equation*}

From $L$ we have
\begin{equation*}
\frac{d}{dt}\frac{\partial L}{\partial\dot x}=m\ddot x,\quad
\frac{\partial L}{\partial x}=0
\end{equation*}

and by Euler-Lagrange
\begin{equation*}
m\ddot x=0
\end{equation*}

Acceleration is zero hence velocity is constant.
Velocity equals distance divided by time.
\begin{equation*}
\dot x=\frac{x_b-x_a}{T}
\end{equation*}

The action is
\begin{align*}
S&=\int_0^TL\,dt
\\
&=\frac{m}{2}\int_0^T\dot x^2\,dt
\\
&=\frac{m}{2}\int_0^T\frac{(x_b-x_a)^2}{T^2}\,dt
\\
&=\left[\frac{m(x_b-x_a)^2}{2T^2}t\right]_{t=0}^{t=T}
\\
&=\frac{m(x_b-x_a)^2}{2T}
\tag{1}
\end{align*}

\end{document}
