\input{preamble}

\section*{Fun trick}

Show that
\begin{equation*}
\left[p^2,\mathbf r\right]=-2i\hbar\mathbf p
\end{equation*}

where
\begin{equation*}
\mathbf r=\otimes(x,y,z),\quad
\mathbf p=-i\hbar\nabla,\quad
p^2=\mathbf p\cdot\mathbf p=-\hbar^2\nabla^2
\end{equation*}

We have
\begin{align*}
[p^2,\mathbf r]
&=p^2\mathbf r-\mathbf rp^2
\\
&=\mathbf p\cdot\mathbf p\mathbf r-\mathbf r \mathbf p\cdot\mathbf p
\\
&=[\mathbf p\mathbf p\mathbf r-\mathbf p\mathbf r\mathbf p]_{1,2}
+[\mathbf p\mathbf r\mathbf p-\mathbf r\mathbf p\mathbf p]_{2,3}
\tag*{\text{trick!}}
\\
&=[\mathbf p(\mathbf{pr}-\mathbf{rp})]_{1,2}+[(\mathbf{pr}-\mathbf{rp})\mathbf p]_{2,3}
\\
&=[\mathbf p(-i\hbar\mathbf I)]_{1,2}+[(-i\hbar\mathbf I)\mathbf p]_{2,3}
\\
&=\mathbf p(-i\hbar)+(-i\hbar)\mathbf p
\\
&=-2i\hbar\mathbf p
\end{align*}

where $[\,]_{i,j}$ means contract on indices $i$ and $j$ and
$\mathbf I$ is the $3\times3$ identity matrix.

\bigskip
Verify the following formulas.
\begin{align*}
[p^2,\mathbf r]
&=-2i\hbar\mathbf p
\tag{1}
\\[1ex]
[p^2,\mathbf r]
&=[\mathbf p\mathbf p\mathbf r-\mathbf p\mathbf r\mathbf p]_{1,2}
+[\mathbf p\mathbf r\mathbf p-\mathbf r\mathbf p\mathbf p]_{2,3}
\tag{2}
\\[1ex]
\mathbf p\mathbf r-\mathbf r\mathbf p&=-i\hbar\mathbf I
\tag{3}
\\[1ex]
\mathbf p\cdot\mathbf p&=[\mathbf p\mathbf p]_{1,2}
\tag{4}
\end{align*}

\end{document}
