\input{preamble}

\section*{Galilean transformation}

Let $U$ be the transformation
\begin{equation*}
U=1-i\epsilon G_1-\tfrac{1}{2}\epsilon^2G_1^2
\end{equation*}

where
\begin{equation*}
G_1=\frac{m}{\hbar}X_1
\end{equation*}

Show that for $\epsilon^4=\epsilon^3=0$ we have
\begin{equation*}
U^{-1}P_1U=P_1-\epsilon m,\quad U^{-1}P_2U=P_2,\quad U^{-1}P_3U=P_3\tag{1}
\end{equation*}

and
\begin{equation*}
U^{-1}HU=H-\epsilon P_1+\tfrac{1}{2}\epsilon^2m\tag{2}
\end{equation*}

where
\begin{equation*}
H=\frac{1}{2m}\left(P_1^2+P_2^2+P_3^2\right)
\end{equation*}

\end{document}
