\input{preamble}

\section*{Harmonic oscillator propagator}

Show that
\begin{equation*}
\left[x^2,p^2\right]=2i\hbar(xp+px)
\tag{1}
\end{equation*}

By the identity
\begin{equation*}
[AB,CD]=A[B,C]D+AC[B,D]+[A,C]DB+C[A,D]B
\end{equation*}

we have
\begin{equation*}
\left[x^2,p^2\right]=[xx,pp]=x[x,p]p+xp[x,p]+[x,p]px+p[x,p]x
\end{equation*}

Substitute $i\hbar$ for $[x,p]$.
\begin{equation*}
\left[x^2,p^2\right]=2i\hbar(xp+px)
\end{equation*}

Show that
\begin{equation*}
\left[x^2,xp+px\right]=4i\hbar x^2
\tag{2}
\end{equation*}

We have
\begin{equation*}
\left[x^2,xp+px\right]=[xx,xp]+[xx,px]
=xx[x,p]+x[x,p]x+x[x,p]x+[x,p]xx
\end{equation*}

Substitute $i\hbar$ for $[x,p]$.
\begin{equation*}
\left[x^2,xp+px\right]=4i\hbar x^2
\end{equation*}

Show that
\begin{equation*}
\left[p^2,xp+px\right]=-4i\hbar p^2
\tag{3}
\end{equation*}

We have
\begin{equation*}
\left[p^2,xp+px\right]=[pp,xp]+[pp,px]
=p[p,x]p+[p,x]pp+pp[p,x]+p[p,x]p
\end{equation*}

Substitute $-i\hbar$ for $[p,x]$.
\begin{equation*}
\left[p^2,xp+px\right]=-4i\hbar p^2
\end{equation*}

\end{document}


\begin{equation*}
\left[x^2,p^2\right]=2i\hbar(xp+px),\quad
\left[x^2,xp+px\right]=4i\hbar x^2,\quad
\left[p^2,xp+px\right]=-4i\hbar p^2
\end{equation*}

\end{document}
