\input{preamble}

\section*{Laguerre polynomials}

Verify
\begin{equation*}
x\frac{d^2}{dx^2}L_{n\alpha}(x)+(\alpha+1-x)\frac{d}{dx}L_{n\alpha}(x)+nL_{n\alpha}(x)=0
\end{equation*}

where $L_{n\alpha}(x)$ is the associated Laguerre polynomial
\begin{equation*}
L_{n\alpha}(x)=\frac{e^x}{x^\alpha n!}\frac{d^n}{dx^n}(x^{n+\alpha}e^{-x})
\end{equation*}

For integer $\alpha$ the following formula can be used.
\begin{equation*}
L_{n\alpha}(x)=(n+\alpha)!\sum_{k=0}^n\frac{(-x)^k}{(n-k)!(\alpha+k)!k!}
\end{equation*}

\end{document}
