\input{preamble}

% see griffiths and schroeter problem 10.8

\section*{Laplacian of product}

Let 
\begin{equation*}
F(\mathbf r)=\frac{e^{ikr}}{r}
\end{equation*}

where $r=|\mathbf r|$.
Show that
\begin{equation*}
\nabla^2F(\mathbf r)=-k^2F(\mathbf r)-4\pi\delta^3(\mathbf r)
\end{equation*}

Recall $\nabla^2=\nabla\cdot\nabla$ and
\begin{equation*}
\nabla\cdot(f\mathbf A)=\nabla f\cdot\mathbf A+f\nabla\cdot\mathbf A
\end{equation*}

Hence
\begin{align*}
\nabla^2F(\mathbf r)
&=\nabla\cdot\nabla\left(\frac{e^{ikr}}{r}\right)
\\
&=\nabla\cdot\left(\frac{1}{r}\nabla e^{ikr}+e^{ikr}\nabla\frac{1}{r}\right)
\\
&=\biggl(
\underset{\text{see (2)}}{\nabla\frac{1}{r}\cdot\nabla e^{ikr}}
+\underset{\text{see (3)}}{\frac{1}{r}\nabla^2e^{ikr}}
+\underset{\text{see (2)}}{\nabla e^{ikr}\cdot\nabla\frac{1}{r}}
+e^{ikr}\nabla^2\frac{1}{r}
\biggr)\tag{1}
\end{align*}

In spherical coordinates
\begin{equation*}
\nabla f=\frac{\partial f}{\partial r}\hat{\mathbf e}_r
+\frac{1}{r}\frac{\partial f}{\partial\theta}\hat{\mathbf e}_\theta
+\frac{1}{r\sin\theta}\frac{\partial f}{\partial\phi}\hat{\mathbf e}_\phi
\end{equation*}

Hence
\begin{equation*}
\nabla\frac{1}{r}\cdot\nabla e^{ikr}
=\left(-\frac{1}{r^2}\hat{\mathbf e}_r+0\hat{\mathbf e}_\theta+0\hat{\mathbf e}_\phi\right)
\cdot\left(ike^{ikr}\hat{\mathbf e}_r+0\hat{\mathbf e}_\theta+0\hat{\mathbf e}_\phi\right)
=-\frac{ike^{ikr}}{r^2}\tag{2}
\end{equation*}

and
\begin{align*}
\frac{1}{r}\nabla^2e^{ikr}&=\frac{1}{r^2}\frac{\partial^2}{\partial r^2}(re^{ikr})
\\
&=\frac{1}{r^2}\frac{\partial}{\partial r}\left(e^{ikr}+ikre^{ikr}\right)
\\
&=\frac{1}{r^2}\left(2ike^{ikr}-k^2re^{ikr}\right)
\\
&=\frac{2ike^{ikr}}{r^2}-\frac{k^2e^{ikr}}{r}\tag{3}
\end{align*}

Substitute (2) and (3) into (1) to obtain
\begin{align*}
\nabla^2F(\mathbf r)&=-\frac{k^2e^{ikr}}{r}+e^{ikr}\nabla^2\frac{1}{r}
\\
&=-k^2F(\mathbf r)-4\pi\delta^3(\mathbf r)e^{ikr}
\end{align*}

Noting that $\delta^3(\mathbf r)$ vanishes for $r\ne0$ and $e^{ikr}=1$ for $r=0$ we have
\begin{equation*}
\nabla^2F(\mathbf r)=-k^2F(\mathbf r)-4\pi\delta^3(\mathbf r)\tag{4}
\end{equation*}

\end{document}
