\input{preamble}

\section*{Laplace transform example}

Solve for $c_a(t)$ and $c_b(t)$ where $c_a(0)=1$, $c_b(0)=0$, and
\begin{align*}
i\hbar\dot c_a(t)&=Ae^{-i\omega t}c_b(t)
\\
i\hbar\dot c_b(t)&=Be^{i\omega t}c_a(t)
\end{align*}

Start with Laplace transforms.
\begin{align*}
i\hbar[sC_a(s)-c_a(0)]&=AC_b(s+i\omega)
\\
i\hbar[sC_b(s)-c_b(0)]&=BC_a(s-i\omega)
\tag{1}
\end{align*}

Solve for $C_a(s)$ with $c_a(0)=1$.
\begin{equation*}
C_a(s)=\frac{AC_b(s+i\omega)+i\hbar}{i\hbar s}
\end{equation*}

Hence
\begin{equation*}
C_a(s-i\omega)=-\frac{iAC_b(s)}{\hbar(s-i\omega)}+\frac{1}{s-i\omega}
\tag{2}
\end{equation*}

Substitute (2) into (1) with $c_b(0)=0$ to obtain
\begin{equation*}
i\hbar sC_b(s)=-\frac{iABC_b(s)}{\hbar(s-i\omega)}+\frac{B}{s-i\omega}
\end{equation*}

Rearrange as
\begin{equation*}
i\hbar sC_b(s)+\frac{iABC_b(s)}{\hbar(s-i\omega)}=\frac{B}{s-i\omega}
\end{equation*}

Rearrange again as
\begin{equation*}
C_b(s)\left[i\hbar s+\frac{iAB}{\hbar(s-i\omega)}\right]=\frac{B}{s-i\omega}
\end{equation*}

Hence
\begin{equation*}
C_b(s)=\frac
{\displaystyle\frac{B}{s-i\omega}}
{\displaystyle i\hbar s+\frac{iAB}{\hbar(s-i\omega)}}
=\frac{-iB/\hbar}{s^2-i\omega s+AB/\hbar^2}
\end{equation*}

Inverse Laplace transform:
\begin{equation*}
\frac{1}{s^2+as+b}\quad\Rightarrow\quad
\frac{2}{k}\sin\left(\frac{kt}{2}\right)\exp\left(-\frac{at}{2}\right),\quad
k=\sqrt{4b-a^2}
\end{equation*}

Hence for $a=-i\omega$ and $b=AB/\hbar^2$ we have
\begin{equation*}
c_b(t)=-\frac{2iB}{\hbar k}
\sin\left(\frac{kt}{2}\right)
\exp\left(\frac{i\omega t}{2}\right),\quad
k=\sqrt{\frac{4AB}{\hbar^2}+\omega^2}
\end{equation*}

Solve for $c_a(t)$.
\begin{equation*}
c_a(t)=\frac{i\hbar\dot c_b(t)}{Be^{i\omega t}}
=\cos\left(\frac{kt}{2}\right)\exp\left(-\frac{i\omega t}{2}\right)
+\frac{i\omega}{k}\sin\left(\frac{kt}{2}\right)\exp\left(-\frac{i\omega t}{2}\right)
\end{equation*}

\end{document}
