\input{preamble}

\section*{Laplace transform example 2}

Let $\hat H(\mathbf r,t)$ be the Hamiltonian
\begin{equation*}
\hat H(\mathbf r,t)=\hat H_0(\mathbf r)+\hat H_1(\mathbf r,t)
\end{equation*}

where
\begin{equation*}
\hat H_0\psi_a=E_a\psi_a,\quad\hat H_0\psi_b=E_b\psi_b,\quad
\hat H_0\Psi=(E_a+E_b)\Psi
\end{equation*}

Let $\Psi(\mathbf r,t)$ be the following wave function for a two state system.
\begin{equation*}
\Psi(\mathbf r,t)=\psi_a(\mathbf r)c_a(t)\exp(-\tfrac{i}{\hbar}E_at)+
\psi_b(\mathbf r)c_b(t)\exp(-\tfrac{i}{\hbar}E_bt)
\end{equation*}

From the Schr\"odinger equation
\begin{equation*}
i\hbar\frac{\partial}{\partial t}\Psi=\hat H\Psi
\end{equation*}

we obtain the differential equations
\begin{align*}
\frac{d}{dt}c_a(t)&=H_{aa}c_a(t)+H_{ab}c_b(t)\exp(-i\omega_0t)
\tag{1}
\\[1ex]
\frac{d}{dt}c_b(t)&=H_{bb}c_b(t)+H_{ba}c_a(t)\exp(i\omega_0t)
\tag{2}
\end{align*}

where
\begin{equation*}
H_{ij}=-\frac{i}{\hbar}\langle\psi_i|\hat H_1|\psi_j\rangle,\quad
\omega_0=\frac{E_b-E_a}{\hbar}
\end{equation*}

Solve equations (1) and (2) with initial conditions $c_a(0)=1$ and $c_b(0)=0$.

\bigskip
Start with the following Laplace transforms for (1) and (2).
\begin{align*}
sC_a(s)-c_a(0)&=H_{aa}C_a(s)+H_{ab}C_b(s+i\omega_0)
\tag{3}
\\
sC_b(s)-c_b(0)&=H_{bb}C_b(s)+H_{ba}C_a(s-i\omega_0)
\tag{4}
\end{align*}

Use equation (3) to solve for $C_a(s)$ with $c_a(0)=1$.
\begin{equation*}
C_a(s)=\frac{H_{ab}C_b(s+i\omega_0)}{s-H_{aa}}+\frac{1}{s-H_{aa}}
\end{equation*}

Solve for $C_a(s-i\omega_0)$.
\begin{equation*}
C_a(s-i\omega)=\frac{H_{ab}C_b(s)}{s-i\omega_0-H_{aa}}+\frac{1}{s-i\omega_0-H_{aa}}
\tag{5}
\end{equation*}

Substitute (5) into (4) to obtain
\begin{equation*}
sC_b(s)-c_b(0)=H_{bb}C_b(s)+H_{ba}
\left(
\frac{H_{ab}C_b(s)}{s-i\omega_0-H_{aa}}+\frac{1}{s-i\omega_0-H_{aa}}
\right)
\end{equation*}

It follows that for $c_b(0)=0$
\begin{equation*}
C_b(s)\left[s-H_{bb}-\frac{H_{ab}H_{ba}}{s-i\omega_0-H_{aa}}\right]=\frac{H_{ba}}{s-i\omega_0-H_{aa}}
\end{equation*}

Hence
\begin{equation*}
C_b(s)=\frac{H_{ba}}{s^2-(H_{aa}+H_{bb}+i\omega_0)s+H_{aa}H_{bb}-H_{ab}H_{ba}+iH_{bb}\omega_0}
\end{equation*}

Inverse Laplace transform:
\begin{equation*}
\frac{1}{s^2+as+b}\quad\Rightarrow\quad
\frac{2}{k}\sin\left(\frac{kt}{2}\right)\exp\left(-\frac{at}{2}\right),\quad
k=\sqrt{4b-a^2}
\end{equation*}

Hence for
\begin{equation*}
a=-(H_{aa}+H_{bb}+i\omega_0),\quad
b=H_{aa}H_{bb}-H_{ab}H_{ba}+iH_{bb}\omega_0
\end{equation*}

we have
\begin{equation*}
c_b(t)=\frac{2H_{ba}}{k}
\sin\left(\frac{kt}{2}\right)
\exp\left(-\frac{at}{2}\right)
\end{equation*}

Use equation (2) to solve for $c_a(t)$.
\begin{equation*}
c_a(t)=\left[
\cos\left(\frac{kt}{2}\right)-\frac{a+2H_{bb}}{k}\sin\left(\frac{kt}{2}\right)
\right]\exp(-i\omega_0t)\exp\left(-\frac{at}{2}\right)
\end{equation*}

For the typical case of $H_{aa}=H_{bb}=0$ we have
\begin{align*}
c_a(t)&=\left[\cos\left(\frac{kt}{2}\right)+\frac{i\omega_0}{k}\sin\left(\frac{kt}{2}\right)\right]
\exp\left(-\frac{i\omega_0t}{2}\right)
\tag{6}
\\[1ex]
c_b(t)&=\frac{2H_{ba}}{k}\sin\left(\frac{kt}{2}\right)\exp\left(\frac{i\omega_0t}{2}\right)
\tag{7}
\end{align*}

\end{document}
