\input{preamble}

\section*{l'H\^opital's rule}

Find the following limit.
\begin{equation*}
y=\lim_{n\rightarrow\infty}\left(1-\frac{\alpha}{n^2}\right)^n
\end{equation*}

Rewrite as
\begin{equation*}
y=\lim_{n\rightarrow\infty}\exp\left[n\log\left(1-\frac{\alpha}{n^2}\right)\right]
\end{equation*}

By composition limit law rewrite as exponential of limit.
\begin{equation*}
y=\exp\left[
\lim_{n\rightarrow\infty}
n\log\left(1-\frac{\alpha}{n^2}\right)
\right]
\end{equation*}

Rewrite again as
\begin{equation*}
y=\lim_{n\rightarrow\infty}\exp\left[\frac{\log\left(1-\frac{\alpha}{n^2}\right)}{\frac{1}{n}}\right]
\end{equation*}

Both numerator and denominator have limit zero hence apply l'H\^opital's rule.
\begin{equation*}
y=\exp\left[
\lim_{n\rightarrow\infty}
\frac{\frac{d}{dn}\log\left(1-\frac{\alpha}{n^2}\right)}
{\frac{d}{dn}\frac{1}{n}}
\right]
=\exp\left(
\lim_{n\rightarrow\infty}
\frac
{\frac{2\alpha}{n^3-\alpha n}}
{-\frac{1}{n^2}}
\right)
\end{equation*}

Hence
\begin{equation*}
y=\exp\left(
\lim_{n\rightarrow\infty}
\frac{2\alpha}{\frac{\alpha}{n}-n}
\right)
=\exp(0)=1
\end{equation*}

\end{document}
