\input{preamble}

\section*{Perturbation example}

Let
\begin{equation*}
\begin{aligned}
\dot c_a&=-\frac{i}{\hbar}c_bH_{ab}e^{-i\omega t}
\\
\dot c_b&=-\frac{i}{\hbar}c_aH_{ba}e^{i\omega t}
\end{aligned}
\end{equation*}

Find $c_a(t)$ and $c_b(t)$ to second order for $c_a(0)=a$ and $c_b(0)=b$.
(See Griffiths and Schroeter problem 11.6.)

\bigskip
First order:
\begin{equation*}
\begin{aligned}
\dot c_a^{(1)}&=-\frac{i}{\hbar}H_{ab}e^{-i\omega t}c_b\bigg|_{c_b=b}
&&=-\frac{ib}{\hbar}H_{ab}e^{-i\omega t}
\\
\dot c_b^{(1)}&=-\frac{i}{\hbar}H_{ba}e^{i\omega t}c_a\bigg|_{c_a=a}
&&=-\frac{ia}{\hbar}H_{ba}e^{i\omega t}
\end{aligned}
\tag{1}
\end{equation*}

Hence
\begin{equation*}
\begin{aligned}
c_a^{(1)}(t)&=a+\int_0^t\dot c_a^{(1)}(t')\,dt'
&&=a-\frac{ib}{\hbar}\int_0^tH_{ab}(t')e^{-i\omega t'}\,dt'
\\
c_b^{(1)}(t)&=b+\int_0^t\dot c_b^{(1)}(t')\,dt'
&&=b-\frac{ia}{\hbar}\int_0^tH_{ba}(t')e^{i\omega t'}\,dt'
\end{aligned}
\tag{2}
\end{equation*}

Second order:
\begin{equation*}
\begin{aligned}
\dot c_a^{(2)}&=-\frac{i}{\hbar}H_{ab}e^{-i\omega t}c_b\bigg|_{c_b=c_b^{(1)}}
&&=-\frac{ib}{\hbar}H_{ab}e^{-i\omega t}-\frac{a}{\hbar^2}H_{ab}e^{-i\omega t}
\int_0^tH_{ba}(t')e^{i\omega t'}\,dt'
\\
\dot c_b^{(2)}&=-\frac{i}{\hbar}H_{ba}e^{i\omega t}c_a\bigg|_{c_a=c_a^{(1)}}
&&=-\frac{ia}{\hbar}H_{ba}e^{i\omega t}-\frac{b}{\hbar^2}H_{ba}e^{i\omega t}
\int_0^tH_{ab}(t')e^{-i\omega t'}\,dt'
\end{aligned}
\tag{3}
\end{equation*}

Hence
\begin{multline*}
c_a^{(2)}(t)=a+\int_0^t\dot c_a^{(2)}(t')\,dt'
\\
=a-\frac{ib}{\hbar}\int_0^tH_{ab}(t')e^{-i\omega t'}\,dt'
-\frac{a}{\hbar^2}\int_0^tH_{ab}(t')e^{-i\omega t'}
\left[\int_0^{t'}H_{ba}(t'')e^{i\omega t''}\,dt''\right]\,dt'
\tag{4}
\end{multline*}

and
\begin{multline*}
c_b^{(2)}(t)=b+\int_0^t\dot c_b^{(2)}(t')\,dt'
\\
=b-\frac{ia}{\hbar}\int_0^tH_{ba}(t')e^{i\omega t'}\,dt'
-\frac{b}{\hbar^2}\int_0^tH_{ba}(t')e^{i\omega t'}
\left[\int_0^{t'}H_{ab}(t'')e^{-i\omega t''}\,dt''\right]\,dt'
\tag{5}
\end{multline*}

\end{document}
