\input{preamble}

\section*{Probability current}

Let $\mathbf J$ be the probability current
\begin{equation*}
\mathbf J=\frac{i\hbar}{2m}\left(\Psi\nabla\Psi^*-\Psi^*\nabla\Psi\right)
\end{equation*}

Show that
\begin{equation*}
\nabla\cdot\mathbf J=-\frac{\partial}{\partial t}|\Psi|^2
\end{equation*}

Recall that
\begin{equation*}
\nabla\cdot\nabla=\nabla^2
\end{equation*}

By the product rule for divergence we have
\begin{equation*}
\nabla\cdot(\Psi\nabla\Psi^*)
=\nabla\Psi\cdot\nabla\Psi^*+\Psi\nabla^2\Psi^*
\end{equation*}

Hence
\begin{equation*}
\nabla\cdot\mathbf J
=\frac{i\hbar}{2m}\left(\Psi\nabla^2\Psi^*-\Psi^*\nabla^2\Psi\right)
\tag{1}
\end{equation*}

For the time derivative we have
\begin{equation*}
\frac{\partial}{\partial t}|\Psi|^2
=\frac{\partial}{\partial t}(\Psi^*\Psi)
=\Psi^*\frac{\partial\Psi}{\partial t}+\Psi\frac{\partial\Psi^*}{\partial t}
\tag{2}
\end{equation*}

Recall the Schr\"odinger equation
\begin{equation*}
\frac{\partial\Psi}{\partial t}
=\frac{i\hbar}{2m}\nabla^2\Psi-\frac{i}{\hbar}V\Psi
\tag{3}
\end{equation*}

Substitute (3) into (2) to obtain
\begin{align*}
\frac{\partial}{\partial t}|\Psi|^2
&=\Psi^*\left(\frac{i\hbar}{2m}\nabla^2\Psi-\frac{i}{\hbar}V\Psi\right)
+\Psi\left(-\frac{i\hbar}{2m}\nabla^2\Psi+\frac{i}{\hbar}V\Psi\right)
\\
&=\frac{i\hbar}{2m}\left(\Psi^*\nabla^2\Psi-\Psi\nabla^2\Psi^*\right)
\tag{4}
\end{align*}

Hence by (1) and (4)
\begin{equation*}
\nabla\cdot\mathbf J=-\frac{\partial}{\partial t}|\Psi|^2
\end{equation*}

\end{document}
