\input{preamble}

\section*{Quantum angular momentum}

For $l=1$ and $l=2$ find the eigenfunctions of $L_x$ where
\begin{equation*}
L_x=i\hbar\left(
\sin\phi\frac{\partial}{\partial\theta}+\cos\phi\cot\theta\frac{\partial}{\partial\phi}
\right)
\end{equation*}

In other words, find the eigenfunctions $\psi_{l,m}$ such that $L_x\psi_{l,m}=m\hbar\psi_{l,m}$.

\bigskip
Using ladder operators we have
\begin{equation*}
L_xY_{l,m}=\tfrac{1}{2}(L_++L_-)Y_{l,m}
=\frac{\hbar}{2}\left(c_{l,m}^+Y_{l,m+1}+c_{l,m}^-Y_{l,m-1}\right)
\end{equation*}

where
\begin{align*}
c_{l,m}^+&=\sqrt{(l-m)(l+m+1)}=\sqrt{l(l+1)-m(m+1)}
\\
c_{l,m}^-&=\sqrt{(l+m)(l-m+1)}=\sqrt{l(l+1)-m(m-1)}
\end{align*}

Hence for $l=1$ we have
\begin{equation*}
\begin{pmatrix}L_xY_{1,1}\\L_xY_{1,0}\\L_xY_{1,-1}\end{pmatrix}
=
\hbar M_x\begin{pmatrix}Y_{1,1}\\Y_{1,0}\\Y_{1,-1}\end{pmatrix}
\end{equation*}

where
\begin{equation*}
M_x=\frac{1}{2}\begin{pmatrix}
0 & c_{1,0}^+ & 0
\\[1ex]
c_{1,1}^- & 0 & c_{1,-1}^+
\\[1ex]
0 & c_{1,0}^- & 0
\end{pmatrix}
=
\begin{pmatrix}
0 & 1/\sqrt2 & 0
\\[1ex]
1/\sqrt2 & 0 & 1/\sqrt2
\\[1ex]
0 & 1/\sqrt2 & 0
\end{pmatrix}
\end{equation*}

These are the eigenvectors $x_m$ of $M_x$ where $m$ is the eigenvalue.
\begin{align*}
x_1&=\begin{pmatrix}\frac{1}{2} & \frac{1}{\sqrt2} & \frac{1}{2}\end{pmatrix}^T, & M_xx_1&=x_1
\\[1ex]
x_0&=\begin{pmatrix}-\frac{1}{\sqrt2} & 0 & \frac{1}{\sqrt2}\end{pmatrix}^T, & M_xx_0&=0
\\[1ex]
x_{-1}&=\begin{pmatrix}-\frac{1}{2} & \frac{1}{\sqrt2} & -\frac{1}{2}\end{pmatrix}^T, & M_xx_{-1}&=-x_{-1}
\end{align*}

Then by
\begin{equation*}
\psi_{1,m}=x_m\cdot\begin{pmatrix}Y_{1,1}\\Y_{1,0}\\Y_{1,-1}\end{pmatrix}
\end{equation*}

we have
\begin{align*}
\psi_{1,1}&=\frac{1}{2}Y_{1,1}+\frac{1}{\sqrt2}Y_{1,0}+\frac{1}{2}Y_{1,-1},
& L_x\psi_{1,1}&=\hbar\psi_{1,1}
\\[1ex]
\psi_{1,0}&=-\frac{1}{\sqrt2}Y_{1,1}+\frac{1}{\sqrt2}Y_{1,-1},
& L_x\psi_{1,0}&=0
\\[1ex]
\psi_{1,-1}&=-\frac{1}{2}Y_{1,1}+\frac{1}{\sqrt2}Y_{1,0}-\frac{1}{2}Y_{1,-1},
& L_x\psi_{1,-1}&=-\hbar\psi_{1,-1}
\end{align*}

For $l=2$
\begin{equation*}
M_x=\frac{1}{2}\begin{pmatrix}
0 & c_{2,1}^+ & 0 & 0 & 0
\\[1ex]
c_{2,2}^- & 0 & c_{2,0}^+ & 0 & 0
\\[1ex]
0 & c_{2,1}^- & 0 & c_{2,-1}^+ & 0
\\[1ex]
0 & 0 & c_{2,0}^- & 0 & c_{2,-2}^+
\\[1ex]
0 & 0 & 0 &c_{2,-1}^- & 0
\end{pmatrix}
=
\begin{pmatrix}
0 & 1 & 0 & 0 & 0
\\[1ex]
1 & 0 & \sqrt{3/2} & 0 & 0
\\[1ex]
0 & \sqrt{3/2} & 0 & \sqrt{3/2} & 0
\\[1ex]
0 & 0 & \sqrt{3/2} & 0 & 1
\\[1ex]
0 & 0 & 0 & 1 & 0
\end{pmatrix}
\end{equation*}

These are the eigenvectors $x_m$ of $M_x$ where $m$ is the eigenvalue.
\begin{align*}
x_2&=\begin{pmatrix}
\frac{1}{4} & \frac{1}{2} & \frac{\sqrt3}{2\sqrt2} & \frac{1}{2} & \frac{1}{4}
\end{pmatrix}^T, & M_xx_2&=2x_2
\\[1ex]
x_1&=\begin{pmatrix}
-\frac{1}{2} & -\frac{1}{2} & 0 & \frac{1}{2} & \frac{1}{2}
\end{pmatrix}^T, & M_xx_1&=x_1
\\[1ex]
x_0&=\begin{pmatrix}
\frac{\sqrt3}{2\sqrt2} & 0 & -\frac{1}{2} & 0 & \frac{\sqrt3}{2\sqrt2}
\end{pmatrix}^T, & M_xx_0&=0
\\[1ex]
x_{-1}&=\begin{pmatrix}
-\frac{1}{2} & \frac{1}{2} & 0 & -\frac{1}{2} & \frac{1}{2}
\end{pmatrix}^T, & M_xx_{-1}&=-x_{-1}
\\[1ex]
x_{-2}&=\begin{pmatrix}
-\frac{1}{4} & \frac{1}{2} & -\frac{\sqrt3}{2\sqrt2} & \frac{1}{2} & -\frac{1}{4}
\end{pmatrix}^T, & M_xx_{-2}&=-2x_{-2}
\end{align*}

Then by
\begin{equation*}
\psi_{2,m}=x_m\cdot\begin{pmatrix}Y_{2,2}\\Y_{2,1}\\Y_{2,0}\\Y_{2,-1}\\Y_{2,-2}\end{pmatrix}
\end{equation*}

we have
\begin{align*}
\psi_{2,2}&=\frac{1}{4}Y_{2,2}+\frac{1}{2}Y_{2,1}+\frac{\sqrt3}{2\sqrt2}Y_{2,0}
+\frac{1}{2}Y_{2,-1}+\frac{1}{4}Y_{2,-2}, & L_x\psi_{2,2}&=2\hbar\psi_{2,2}
\\[1ex]
\psi_{2,1}&=-\frac{1}{2}Y_{2,2}-\frac{1}{2}Y_{2,1}
+\frac{1}{2}Y_{2,-1}+\frac{1}{2}Y_{2,-2}, & L_x\psi_{2,1}&=\hbar\psi_{2,1}
\\[1ex]
\psi_{2,0}&=\frac{\sqrt3}{2\sqrt2}Y_{2,2}
-\frac{1}{2}Y_{2,0}+\frac{\sqrt3}{2\sqrt2}Y_{2,-2}, & L_x\psi_{2,0}&=0
\\[1ex]
\psi_{2,-1}&=-\frac{1}{2}Y_{2,2}+\frac{1}{2}Y_{2,1}
-\frac{1}{2}Y_{2,-1}+\frac{1}{2}Y_{2,-2}, & L_x\psi_{2,-1}&=-\hbar\psi_{2,-1}
\\[1ex]
\psi_{2,-2}&=-\frac{1}{4}Y_{2,2}+\frac{1}{2}Y_{2,1}-\frac{\sqrt3}{2\sqrt2}Y_{2,0}
+\frac{1}{2}Y_{2,-1}-\frac{1}{4}Y_{2,-2}, & L_x\psi_{2,-2}&=-2\hbar\psi_{2,-2}
\end{align*}

\end{document}
