\input{preamble}

\section*{Quantum angular momentum 1}

Definitions.
\begin{gather*}
\mathbf L=\mathbf X\times\mathbf P
=\begin{pmatrix}
X_2P_3-X_3P_2
\\
X_3P_1-X_1P_3
\\
X_1P_2-X_2P_1
\end{pmatrix}
\\[1ex]
L^2=|\mathbf L|^2={L_1}^2+{L_2}^2+{L_3}^2
\\[1ex]
\mathbf J=\frac{1}{\hbar}\mathbf L
\end{gather*}

Let
\begin{equation*}
X_j=x_j,\quad P_j=-i\hbar\frac{\partial}{\partial x_j}
\end{equation*}

Verify the following formulas where $\psi\equiv\psi(x_1,x_2,x_3,t)$.
\begin{gather*}
%
[\mathbf X,L_3]\psi
=\begin{pmatrix}
-i\hbar X_2
\\
i\hbar X_1
\\
0
\end{pmatrix}\psi
\tag{1}
\\[1ex]
%
[\mathbf P,L_3]\psi
=\begin{pmatrix}
-i\hbar P_2
\\
i\hbar P_1
\\
0
\end{pmatrix}\psi
\tag{2}
\\[1ex]
%
[\mathbf L,L^2]\psi=0
\tag{3}
\\[1ex]
%
\mathbf J\times\mathbf J\psi=i\mathbf J\psi
\tag{4}
\\[1ex]
%
(\mathbf P\times\mathbf L+\mathbf L\times\mathbf P)\psi=2i\hbar\mathbf P\psi
\tag{5}
\\[1ex]
%
\tfrac{1}{2}(\mathbf P\times\mathbf L-\mathbf L\times\mathbf P)\psi
=(\mathbf P\times\mathbf L-i\hbar\mathbf P)\psi
\tag{6}
\\[1ex]
%
[L_i,P_j]\psi=i\hbar\sum_k\epsilon_{ijk}P_k\psi
\tag{7}
\end{gather*}

\end{document}
