\input{preamble}

\section*{Spin operators from scratch}

By definition of expectation value we have
\begin{equation*}
\langle S_x\rangle=\tfrac{\hbar}{2}\Pr\left(\tfrac{\hbar}{2}\right)
+\left(-\tfrac{\hbar}{2}\right)\Pr\left(-\tfrac{\hbar}{2}\right)
\end{equation*}

Rewrite probability as amplitude squared.
\begin{equation*}
\langle S_x\rangle=\tfrac{\hbar}{2}\bigl|\langle x_+|s\rangle\bigr|^2
-\tfrac{\hbar}{2}\bigl|\langle x_-|s\rangle\bigr|^2
\end{equation*}

Equivalently
\begin{equation*}
\langle S_x\rangle
=\tfrac{\hbar}{2}\langle s|x_+\rangle\langle x_+|s\rangle
-\tfrac{\hbar}{2}\langle s|x_-\rangle\langle x_-|s\rangle
\end{equation*}

Factor out spin state $|s\rangle$.
\begin{equation*}
\langle S_x\rangle=\langle s|\Bigl(
\tfrac{\hbar}{2}|x_+\rangle\langle x_+|-\tfrac{\hbar}{2}|x_-\rangle\langle x_-|
\Bigr)|s\rangle
\end{equation*}

Rewrite as
\begin{equation*}
\langle S_x\rangle=\langle s|S_x|s\rangle
\end{equation*}

where
\begin{equation*}
S_x=\tfrac{\hbar}{2}|x_+\rangle\langle x_+|-\tfrac{\hbar}{2}|x_-\rangle\langle x_-|
\end{equation*}

From basis states
\begin{equation*}
x_+=\frac{1}{\sqrt2}\begin{pmatrix}1\\1\end{pmatrix},\quad
x_-=\frac{1}{\sqrt2}\begin{pmatrix}1\\-1\end{pmatrix}
\end{equation*}

we have outer products
\begin{equation*}
|x_+\rangle\langle x_+|=\frac{1}{2}\begin{pmatrix}1&1\\1&1\end{pmatrix},\quad
|x_-\rangle\langle x_-|=\frac{1}{2}\begin{pmatrix}1&-1\\-1&1\end{pmatrix}
\end{equation*}

Hence
\begin{equation*}
S_x=\frac{\hbar}{4}\begin{pmatrix}1&1\\1&1\end{pmatrix}
-\frac{\hbar}{4}\begin{pmatrix}1&-1\\-1&1\end{pmatrix}
=\frac{\hbar}{2}\begin{pmatrix}0&1\\1&0\end{pmatrix}
\end{equation*}

Repeat for $S_y$ and $S_z$.

\end{document}
