\input{preamble}

\section*{Spin direction vector}

Expectation of spin operators is a projection of spin state $|s\rangle$ onto Euclidean space.
\begin{equation*}
\langle x\rangle=\langle s|\sigma_x|s\rangle,
\quad
\langle y\rangle=\langle s|\sigma_y|s\rangle,
\quad
\langle z\rangle=\langle s|\sigma_z|s\rangle
\end{equation*}

Hence the spin direction vector is
\begin{equation*}
\mathbf u=\begin{pmatrix}\langle x\rangle\\\langle y\rangle\\\langle z\rangle\end{pmatrix}
=\langle s|\boldsymbol\sigma|s\rangle,
\quad
\boldsymbol\sigma=\begin{pmatrix}\sigma_x\\\sigma_y\\\sigma_z\end{pmatrix}
\end{equation*}

Let
\begin{equation*}
|s\rangle=\begin{pmatrix}\cos(\theta/2)\\\sin(\theta/2)\exp(i\phi)\end{pmatrix}
\end{equation*}

Then
\begin{equation*}
\langle x\rangle=\sin\theta\cos\phi,\quad
\langle y\rangle=\sin\theta\sin\phi,\quad
\langle z\rangle=\cos\theta
\end{equation*}

and
\begin{equation*}
\cos(\theta/2)=\sqrt{\frac{\langle z\rangle+1}{2}},\quad
\sin(\theta/2)\exp(i\phi)=\sqrt{\frac{1-\langle z\rangle}{2}}
\frac{\langle x\rangle+i\langle y\rangle}{\sqrt{\langle x\rangle^2+\langle y\rangle^2}}
\end{equation*}

Example. Let
\begin{equation*}
|s\rangle=\begin{pmatrix}\frac{1}{3}-\frac{2}{3}i\\[1ex]\frac{2}{3}\end{pmatrix}
\end{equation*}

Then
\begin{equation*}
\mathbf u
=\begin{pmatrix}\langle x\rangle\\\langle y\rangle\\\langle z\rangle\end{pmatrix}
=\begin{pmatrix}\frac{4}{9}\\[1ex]\frac{8}{9}\\[1ex]\frac{1}{9}\end{pmatrix}
\end{equation*}

and
\begin{equation*}
\cos(\theta/2)=\sqrt{\frac{\langle z\rangle+1}{2}}=\frac{\sqrt5}{3},\quad
\sin(\theta/2)\exp(i\phi)=\sqrt{\frac{1-\langle z\rangle}{2}}
\frac{\langle x\rangle+i\langle y\rangle}{\sqrt{\langle x\rangle^2+\langle y\rangle^2}}
=\frac{2+4i}{3\sqrt5}
\end{equation*}

The last result differs from $|s\rangle$ but does represent the same state as $|s\rangle$.

\bigskip
The spin eigenstates are
\begin{align*}
|x_+\rangle&=\tfrac{1}{\sqrt2}(1,1) &
|y_+\rangle&=\tfrac{1}{\sqrt2}(1,i) &
|z_+\rangle&=(1,0)
\\
|x_-\rangle&=\tfrac{1}{\sqrt2}(1,-1) &
|y_-\rangle&=\tfrac{1}{\sqrt2}(1,-i) &
|z_-\rangle&=(0,1)
\end{align*}

Hence for
\begin{equation*}
|s\rangle=\begin{pmatrix}\cos(\theta/2)\\\sin(\theta/2)\exp(i\phi)\end{pmatrix}
\end{equation*}

we have
\begin{align*}
\Pr\left(S_x=+\tfrac{\hbar}{2}\right)
&=|\langle x_+|s\rangle|^2=\tfrac{1}{2}+\tfrac{1}{2}\sin\theta\cos\phi
\\
\Pr\left(S_x=-\tfrac{\hbar}{2}\right)
&=|\langle x_-|s\rangle|^2=\tfrac{1}{2}-\tfrac{1}{2}\sin\theta\cos\phi
\\
\\
\Pr\left(S_y=+\tfrac{\hbar}{2}\right)
&=|\langle y_+|s\rangle|^2=\tfrac{1}{2}+\tfrac{1}{2}\sin\theta\sin\phi
\\
\Pr\left(S_y=-\tfrac{\hbar}{2}\right)
&=|\langle y_-|s\rangle|^2=\tfrac{1}{2}-\tfrac{1}{2}\sin\theta\sin\phi
\\
\\
\Pr\left(S_z=+\tfrac{\hbar}{2}\right)
&=|\langle z_+|s\rangle|^2=\cos^2(\theta/2)
\\
\Pr\left(S_z=-\tfrac{\hbar}{2}\right)
&=|\langle z_-|s\rangle|^2=\sin^2(\theta/2)
\end{align*}

\end{document}
