\input{preamble}

\section*{Spin}

Spin state $|s\rangle$ is a normalized vector in $\mathbb C^2$.
\begin{equation*}
|s\rangle=\begin{pmatrix}c_+\\c_-\end{pmatrix},\quad|c_+|^2+|c_-|^2=1
\end{equation*}

Spin measurement probabilities are the transition probabilities from $|s\rangle$ to an eigenstate.

\bigskip
For spin measurements in the $z$ direction we have
\begin{align*}
\Pr\left(S_z=+\tfrac{\hbar}{2}\right)&=|\langle z_+|s\rangle|^2=|c_+|^2
\\
\Pr\left(S_z=-\tfrac{\hbar}{2}\right)&=|\langle z_-|s\rangle|^2=|c_-|^2
\end{align*}

where the eigenstates are
\begin{equation*}
|z_+\rangle=\begin{pmatrix}1\\0\end{pmatrix},\quad
|z_-\rangle=\begin{pmatrix}0\\1\end{pmatrix}
\end{equation*}

By definition of expectation value we have
\begin{equation*}
\langle S_z\rangle
=\tfrac{\hbar}{2}\Pr\left(S_z=+\tfrac{\hbar}{2}\right)
-\tfrac{\hbar}{2}\Pr\left(S_z=-\tfrac{\hbar}{2}\right)
\end{equation*}

Rewrite as
\begin{equation*}
\langle S_z\rangle=\tfrac{\hbar}{2}|\langle z_+|s\rangle|^2-\tfrac{\hbar}{2}|\langle z_-|s\rangle|^2
\end{equation*}

Rewrite again as
\begin{equation*}
\langle S_z\rangle
=\tfrac{\hbar}{2}\langle s|z_+\rangle\langle z_+|s\rangle
-\tfrac{\hbar}{2}\langle s|z_-\rangle\langle z_-|s\rangle
\end{equation*}

Then by
\begin{equation*}
\langle S_z\rangle=\langle s|S_z|s\rangle
\end{equation*}

we have
\begin{equation*}
S_z=\tfrac{\hbar}{2}|z_+\rangle\langle z_+|-\tfrac{\hbar}{2}|z_-\rangle\langle z_-|
=\frac{\hbar}{2}\begin{pmatrix}1&0\\0&-1\end{pmatrix}
\end{equation*}

From the commutator
\begin{equation*}
S_+S_--S_-S_+=2\hbar S_z
\end{equation*}

we have
\begin{equation*}
S_+S_--S_-S_+
=\hbar^2|z_+\rangle\langle z_+|-\hbar^2|z_-\rangle\langle z_-|
\end{equation*}

Rewrite as
\begin{equation*}
S_+S_--S_-S_+
=\hbar^2|z_+\rangle\langle z_-|z_-\rangle\langle z_+|
-\hbar^2|z_-\rangle\langle z_+|z_+\rangle\langle z_-|
\end{equation*}

Hence
\begin{align*}
S_+&=\hbar|z_+\rangle\langle z_-|=\hbar\begin{pmatrix}0&1\\0&0\end{pmatrix}
\\
S_-&=\hbar|z_-\rangle\langle z_+|=\hbar\begin{pmatrix}0&0\\1&0\end{pmatrix}
\end{align*}

Then by
\begin{align*}
S_+&=S_x+iS_y
\\
S_-&=S_x-iS_y
\end{align*}

we obtain
\begin{align*}
S_x&=\frac{S_++S_-}{2}=\frac{\hbar}{2}\begin{pmatrix}0&1\\1&0\end{pmatrix}
\\
S_y&=\frac{S_+-S_-}{2i}=\frac{\hbar}{2}\begin{pmatrix}0&-i\\i&0\end{pmatrix}
\end{align*}

By solving for the eigenstates in
\begin{align*}
S_x|x_\pm\rangle&=\pm\tfrac{\hbar}{2}|x_\pm\rangle
\\
S_y|y_\pm\rangle&=\pm\tfrac{\hbar}{2}|y_\pm\rangle
\end{align*}

we obtain
\begin{align*}
|x_+\rangle&=\frac{|z_+\rangle+|z_-\rangle}{\sqrt2}=\frac{1}{\sqrt2}\begin{pmatrix}1\\1\end{pmatrix}
\\
|x_-\rangle&=\frac{|z_+\rangle-|z_-\rangle}{\sqrt2}=\frac{1}{\sqrt2}\begin{pmatrix}1\\-1\end{pmatrix}
\end{align*}

and
\begin{align*}
|y_+\rangle&=\frac{|z_+\rangle+i|z_-\rangle}{\sqrt2}=\frac{1}{\sqrt2}\begin{pmatrix}1\\i\end{pmatrix}
\\
|y_-\rangle&=\frac{|z_+\rangle-i|z_-\rangle}{\sqrt2}=\frac{1}{\sqrt2}\begin{pmatrix}1\\-i\end{pmatrix}
\end{align*}

Expectation values for spin operators.
\begin{align*}
\langle S_x\rangle&=\langle s|S_x|s\rangle=\frac{\hbar}{2}\left(c_+c_-^*+c_+^*c_-\right)
\\
\langle S_y\rangle&=\langle s|S_y|s\rangle=\frac{i\hbar}{2}\left(c_+c_-^*-c_+^*c_-\right)
\\
\langle S_z\rangle&=\langle s|S_z|s\rangle=\frac{\hbar}{2}\left(c_+c_+^*-c_-c_-^*\right)
\end{align*}

Expected spin vector.
\begin{equation*}
\langle\mathbf S\rangle=\begin{pmatrix}
\langle S_x\rangle\\
\langle S_y\rangle\\
\langle S_z\rangle
\end{pmatrix}
\end{equation*}

Consider the case of having determined $\langle\mathbf S\rangle$ by experiment.
To convert $\langle\mathbf S\rangle$ to a spin state $|s\rangle$, let
\begin{align*}
x&=\frac{2}{\hbar}\langle S_x\rangle=\sin\theta\cos\phi
\\
y&=\frac{2}{\hbar}\langle S_y\rangle=\sin\theta\sin\phi
\\
z&=\frac{2}{\hbar}\langle S_z\rangle=\cos\theta
\end{align*}

Then
\begin{equation*}
|s\rangle=\begin{pmatrix}\cos(\theta/2)\\\sin(\theta/2)\exp(i\phi)\end{pmatrix}
\end{equation*}

where
\begin{align*}
\cos(\theta/2)&=\sqrt{\frac{\cos\theta+1}{2}}=\sqrt{\frac{z+1}{2}}
\\
\sin(\theta/2)&=\sqrt{\frac{1-\cos\theta}{2}}=\sqrt{\frac{1-z}{2}}
\end{align*}

and
\begin{equation*}
\exp(i\phi)=\cos\phi+i\sin\phi=\frac{x+iy}{\sqrt{x^2+y^2}}
\end{equation*}

The following commutator was used to derive $S_x$ and $S_y$.
\begin{equation*}
S_+S_--S_-S_+=2\hbar S_z
\end{equation*}

The commutator is a consequence of the following wave equation for spin.
\begin{equation*}
\hat{\mathbf S}\psi=(\mathbf r\times\hat{\mathbf p})\psi,\quad
\mathbf r=\begin{pmatrix}x\\y\\z\end{pmatrix},\quad
\hat{\mathbf p}=-i\hbar\begin{pmatrix}
\frac{\partial}{\partial x}
\\
\frac{\partial}{\partial y}
\\
\frac{\partial}{\partial z}
\end{pmatrix}
\end{equation*}

Rewrite in component form.
\begin{align*}
\hat S_x\psi&=-i\hbar\left(y\frac{\partial}{\partial z}-z\frac{\partial}{\partial y}\right)\psi
\\
\hat S_y\psi&=-i\hbar\left(z\frac{\partial}{\partial x}-x\frac{\partial}{\partial z}\right)\psi
\\
\hat S_z\psi&=-i\hbar\left(x\frac{\partial}{\partial y}-y\frac{\partial}{\partial x}\right)\psi
\end{align*}

By computer algebra we have
\begin{align*}
(\hat S_y\hat S_z-\hat S_z\hat S_y)\psi&=i\hbar\hat S_x\psi
\\
(\hat S_z\hat S_x-\hat S_x\hat S_z)\psi&=i\hbar\hat S_y\psi
\\
(\hat S_x\hat S_y-\hat S_y\hat S_x)\psi&=i\hbar\hat S_z\psi
\end{align*}

Let
\begin{align*}
\hat S_+&=\hat S_x+i\hat S_y
\\
\hat S_-&=\hat S_x-i\hat S_y
\end{align*}

By computer algebra
\begin{equation*}
(\hat S_+\hat S_--\hat S_-\hat S_+)\psi=2\hbar\hat S_z\psi
\end{equation*}

\subsubsection*{Exercises}

1. Verify that
\begin{align*}
S_x&=\frac{\hbar}{2}\left(|x_+\rangle\langle x_+|-|x_-\rangle\langle x_-|\right)
\\
S_y&=\frac{\hbar}{2}\left(|y_+\rangle\langle y_+|-|y_-\rangle\langle y_-|\right)
\\
S_z&=\frac{\hbar}{2}\left(|z_+\rangle\langle z_+|-|z_-\rangle\langle z_-|\right)
\end{align*}

2. Let $|s\rangle$ be the following spin state.
\begin{equation*}
|s\rangle=\begin{pmatrix}\frac{1}{3}-\frac{2}{3}i\\[1ex]\frac{2}{3}\end{pmatrix}
\end{equation*}

Verify that $|s\rangle$ is normalized and that
\begin{equation*}
\langle\mathbf S\rangle
=\langle s|\mathbf S|s\rangle
=\frac{\hbar}{2}\begin{pmatrix}\frac{4}{9}\\[1ex]\frac{8}{9}\\[1ex]\frac{1}{9}\end{pmatrix}
\end{equation*}

where
\begin{equation*}
\mathbf S=\begin{pmatrix}S_x\\S_y\\S_z\end{pmatrix}
\end{equation*}

Note: In component form we have
\begin{equation*}
\langle s|\mathbf S|s\rangle
=s_\beta^*{S^{\alpha\beta}}_\gamma s^\gamma
\end{equation*}

Eigenmath requires a transpose so that the $\beta$ indices are adjacent.
\begin{equation*}
\langle s|\mathbf S|s\rangle
=s_\beta^*{S^{\beta\alpha}}_\gamma s^\gamma
\end{equation*}

3. Let $|s\rangle$ be the following spin state.
\begin{equation*}
|s\rangle=\begin{pmatrix}\frac{1}{3}-\frac{2}{3}i\\[1ex]\frac{2}{3}\end{pmatrix}
\end{equation*}

Verify the following measurement probabilities for $|s\rangle$.
\begin{align*}
\Pr\left(S_x=+\tfrac{\hbar}{2}\right)&=|\langle x_+|s\rangle|^2=\tfrac{13}{18}
\\
\Pr\left(S_x=-\tfrac{\hbar}{2}\right)&=|\langle x_-|s\rangle|^2=\tfrac{5}{18}
\\[1ex]
\Pr\left(S_y=+\tfrac{\hbar}{2}\right)&=|\langle y_+|s\rangle|^2=\tfrac{17}{18}
\\
\Pr\left(S_y=-\tfrac{\hbar}{2}\right)&=|\langle y_-|s\rangle|^2=\tfrac{1}{18}
\\[1ex]
\Pr\left(S_z=+\tfrac{\hbar}{2}\right)&=|\langle z_+|s\rangle|^2=\tfrac{5}{9}
\\
\Pr\left(S_z=-\tfrac{\hbar}{2}\right)&=|\langle z_-|s\rangle|^2=\tfrac{4}{9}
\end{align*}

4. Let $|s\rangle$ be the following spin state.
\begin{equation*}
|s\rangle=\begin{pmatrix}\frac{1}{3}-\frac{2}{3}i\\[1ex]\frac{2}{3}\end{pmatrix}
\end{equation*}

Verify that for $\theta$ and $\phi$ determined by $|s\rangle$,
the following spin state $|\chi\rangle$ is indistinguishable from $|s\rangle$.
\begin{equation*}
|\chi\rangle
=\begin{pmatrix}\cos(\theta/2)\\\sin(\theta/2)\exp(i\phi)\end{pmatrix}
=\begin{pmatrix}\frac{\sqrt5}{3}\\[1ex]\frac{2+4i}{3\sqrt5}\end{pmatrix}
\end{equation*}

5. Verify the following commutators for the wave equation
$\mathbf S\psi=(\mathbf r\times\mathbf p)\psi$.
\begin{align*}
[S_y,S_z]&=i\hbar S_x
\\
[S_z,S_x]&=i\hbar S_y
\\
[S_x,S_y]&=i\hbar S_z
\\[1ex]
[S_+,S_-]&=2\hbar S_z
\end{align*}

\end{document}
