\input{preamble}

% http://kirkmcd.princeton.edu/examples/dirac.pdf

% Lancaster and Blundell p. 333 "In fact, the Dirac equation is correctly interpreted as providing the equation of motion for fermionic quantum fields."

\section*{Spinor boost}

This vector represents an electron at rest with spin up along the $z$ axis.
\begin{equation*}
u^0=\sqrt{2m}\begin{pmatrix}1\\0\\0\\0\end{pmatrix}
\end{equation*}

This matrix boosts a spinor in the $z$ direction where $E^2=p^2+m^2$.
\begin{equation*}
\Lambda=\frac{1}{\sqrt{2m(E+m)}}
\begin{pmatrix}
E+m & 0 & p & 0\\
0 & E+m & 0 & p\\
p & 0 & E+m & 0\\
0 & p & 0 & E+m\\
\end{pmatrix}
\end{equation*}

Hence
\begin{equation*}
u=\Lambda u^0=\frac{1}{\sqrt{E+m}}
\begin{pmatrix}
E+m & 0 & p & 0\\
0 & E+m & 0 & p\\
p & 0 & E+m & 0\\
0 & p & 0 & E+m\\
\end{pmatrix}
\begin{pmatrix}1\\0\\0\\0\end{pmatrix}
=\frac{1}{\sqrt{E+m}}\begin{pmatrix}E+m\\0\\p\\0\end{pmatrix}
\end{equation*}

Consider the Dirac equation
\begin{equation*}
\slashed pu=mu
\end{equation*}

Rewrite $u$ as boost.
\begin{equation*}
\slashed p\Lambda u^0=m\Lambda u^0
\end{equation*}

Noting that $\gamma^0u^0=u^0$ we can write
\begin{equation*}
\slashed p\Lambda u^0=m\Lambda\gamma^0u^0
\end{equation*}

Rewrite $u^0$ as boost.
\begin{equation*}
\slashed p\Lambda\Lambda^{-1}u=m\Lambda\gamma^0\Lambda^{-1}u
\end{equation*}

Hence
\begin{equation*}
\slashed p=m\Lambda\gamma^0\Lambda^{-1}
\end{equation*}

and
\begin{equation*}
\Lambda\gamma^0=m^{-1}\slashed p\Lambda
\tag{1}
\end{equation*}

Consider
\begin{equation*}
\gamma^0u^0-u^0=0
\end{equation*}

Apply boost to recover the Dirac equation.
\begin{align*}
\Lambda(\gamma^0u^0-u^0)&=m^{-1}\slashed p\Lambda u^0-\Lambda u^0=m^{-1}\slashed pu-u=0
\tag{2}
\end{align*}

\end{document}
