\input{preamble}

\section*{Two spins}

Spin state $|s\rangle$ for two spins is a unit vector in $\mathbb C^4$.
\begin{equation*}
|s\rangle=\begin{pmatrix}c_{++}\\c_{+-}\\c_{-+}\\c_{--}\end{pmatrix},\quad
|c_{++}|^2+|c_{+-}|^2+|c_{-+}|^2+|c_{--}|^2=1
\end{equation*}

Spin measurement probabilities are the transition probabilities from $|s\rangle$
to an eigenstate.

\bigskip
For spin measurements in the $z$ direction we have
\begin{align*}
\Pr\left(S_{1z}=+\tfrac{\hbar}{2}\text{ and }S_{2z}=+\tfrac{\hbar}{2}\right)
&=|\langle z_{++}|s\rangle|^2=|c_{++}|^2
\\
\Pr\left(S_{1z}=+\tfrac{\hbar}{2}\text{ and }S_{2z}=-\tfrac{\hbar}{2}\right)
&=|\langle z_{+-}|s\rangle|^2=|c_{+-}|^2
\\
\Pr\left(S_{1z}=-\tfrac{\hbar}{2}\text{ and }S_{2z}=+\tfrac{\hbar}{2}\right)
&=|\langle z_{-+}|s\rangle|^2=|c_{-+}|^2
\\
\Pr\left(S_{1z}=-\tfrac{\hbar}{2}\text{ and }S_{2z}=-\tfrac{\hbar}{2}\right)
&=|\langle z_{--}|s\rangle|^2=|c_{--}|^2
\end{align*}

where the eigenstates are
\begin{equation*}
z_{++}=\begin{pmatrix}1\\0\\0\\0\end{pmatrix},\quad
z_{+-}=\begin{pmatrix}0\\1\\0\\0\end{pmatrix},\quad
z_{-+}=\begin{pmatrix}0\\0\\1\\0\end{pmatrix},\quad
z_{--}=\begin{pmatrix}0\\0\\0\\1\end{pmatrix}
\end{equation*}

Spin operators for the first spin
($\otimes$ is kronecker product).
\begin{align*}
S_{1x}&=\frac{\hbar}{2}\sigma_x\otimes I=\frac{\hbar}{2}
\begin{pmatrix}
0&0&1&0\\
0&0&0&1\\
1&0&0&0\\
0&1&0&0
\end{pmatrix}
\\
S_{1y}&=\frac{\hbar}{2}\sigma_y\otimes I=\frac{\hbar}{2}
\begin{pmatrix}
0&0&-i&0\\
0&0&0&-i\\
i&0&0&0\\
0&i&0&0
\end{pmatrix}
\\
S_{1z}&=\frac{\hbar}{2}\sigma_z\otimes I=\frac{\hbar}{2}
\begin{pmatrix}
1&0&0&0\\
0&1&0&0\\
0&0&-1&0\\
0&0&0&-1
\end{pmatrix}
\end{align*}

Spin operators for the second spin.
\begin{align*}
S_{2x}&=\frac{\hbar}{2}I\otimes\sigma_x=\frac{\hbar}{2}
\begin{pmatrix}
0&1&0&0\\
1&0&0&0\\
0&0&0&1\\
0&0&1&0
\end{pmatrix}
\\
S_{2y}&=\frac{\hbar}{2}I\otimes\sigma_y=\frac{\hbar}{2}
\begin{pmatrix}
0&-i&0&0\\
i&0&0&0\\
0&0&0&-i\\
0&0&i&0
\end{pmatrix}
\\
S_{2z}&=\frac{\hbar}{2}I\otimes\sigma_z=\frac{\hbar}{2}
\begin{pmatrix}
1&0&0&0\\
0&-1&0&0\\
0&0&1&0\\
0&0&0&-1
\end{pmatrix}
\end{align*}

Expectation values for the first spin.
\begin{align*}
\langle S_{1x}\rangle&=\langle s|S_{1x}|s\rangle
=\frac{\hbar}{2}
\left(c_{++}c_{-+}^*+c_{++}^*c_{-+}+c_{+-}c_{--}^*+c_{+-}^*c_{--}\right)
\\
\langle S_{1y}\rangle&=\langle s|S_{1y}|s\rangle
=\frac{i\hbar}{2}
\left(c_{++}c_{-+}^*-c_{++}^*c_{-+}+c_{+-}c_{--}^*-c_{+-}^*c_{--}\right)
\\
\langle S_{1z}\rangle&=\langle s|S_{1z}|s\rangle
=\frac{\hbar}{2}
\left(|c_{++}|^2+|c_{+-}|^2-|c_{-+}|^2-|c_{--}|^2\right)
\end{align*}

Expectation values for the second spin.
\begin{align*}
\langle S_{2x}\rangle&=\langle s|S_{2x}|s\rangle
=\frac{\hbar}{2}
\left(c_{++}c_{+-}^*+c_{++}^*c_{+-}+c_{-+}c_{--}^*+c_{-+}^*c_{--}\right)
\\
\langle S_{2y}\rangle&=\langle s|S_{2y}|s\rangle
=\frac{i\hbar}{2}
\left(c_{++}c_{+-}^*-c_{++}^*c_{+-}+c_{-+}c_{--}^*-c_{-+}^*c_{--}\right)
\\
\langle S_{2z}\rangle&=\langle s|S_{2z}|s\rangle
=\frac{\hbar}{2}
\left(|c_{++}|^2-|c_{+-}|^2+|c_{-+}|^2-|c_{--}|^2\right)
\end{align*}

Expected spin vectors.
\begin{equation*}
\langle\mathbf S_1\rangle=\langle s|\mathbf S_1|s\rangle
=\begin{pmatrix}
\langle S_{1x}\rangle\\
\langle S_{1y}\rangle\\
\langle S_{1z}\rangle
\end{pmatrix},\quad
\langle\mathbf S_2\rangle=\langle s|\mathbf S_2|s\rangle
=\begin{pmatrix}
\langle S_{2x}\rangle\\
\langle S_{2y}\rangle\\
\langle S_{2z}\rangle
\end{pmatrix}
\end{equation*}

Consider the case of having determined $\langle\mathbf S_1\rangle$ and
$\langle\mathbf S_2\rangle$ by experiment.
To convert $\langle\mathbf S_1\rangle$ and $\langle\mathbf S_2\rangle$
to a spin state $|s\rangle$, let
\begin{align*}
x_i&=\frac{2}{\hbar}\langle S_{ix}\rangle=\sin\theta_i\cos\phi_i
\\
y_i&=\frac{2}{\hbar}\langle S_{iy}\rangle=\sin\theta_i\sin\phi_i
\\
z_i&=\frac{2}{\hbar}\langle S_{iz}\rangle=\cos\theta_i
\end{align*}

Then
\begin{equation*}
|s_i\rangle=\begin{pmatrix}\cos(\theta_i/2)\\\sin(\theta_i/2)\exp(i\phi_i)\end{pmatrix}
\end{equation*}

where
\begin{align*}
\cos(\theta_i/2)=\sqrt{\frac{\cos\theta_i+1}{2}}=\sqrt{\frac{z_i+1}{2}}
\\
\sin(\theta_i/2)=\sqrt{\frac{1-\cos\theta_i}{2}}=\sqrt{\frac{1-z_i}{2}}
\end{align*}

and
\begin{equation*}
\exp(i\phi_i)=\cos\phi_i+i\sin\phi_i
=\frac{x_i+iy_i}{\sqrt{x_i^2+y_i^2}}
\end{equation*}

Spin state $|s\rangle$ is the kronecker product of $|s_1\rangle$ and $|s_2\rangle$.
\begin{equation*}
|s\rangle=|s_1\rangle\otimes|s_2\rangle
\end{equation*}

Spin total angular momentum magnitude squared operator $(\mathbf S_1+\mathbf S_2)^2$.
\begin{equation*}
(\mathbf S_1+\mathbf S_2)^2
=(S_{1x}+S_{2x})^2+(S_{1y}+S_{2y})^2+(S_{1z}+S_{2z})^2
=\hbar^2\begin{pmatrix}
2&0&0&0\\
0&1&1&0\\
0&1&1&0\\
0&0&0&2
\end{pmatrix}
\end{equation*}

Expectation value for $(\mathbf S_1+\mathbf S_2)^2$.
\begin{equation*}
\langle s|(\mathbf S_1+\mathbf S_2)^2|s\rangle
=\hbar^2\left(2|c_{++}|^2+|c_{+-}+c_{-+}|^2+2|c_{--}|^2\right)
\end{equation*}

\subsubsection*{Exercises}

1. Verify spin operators for two spins.

\bigskip
2. Verify expectation values for two spins.

\bigskip
3. Let
\begin{equation*}
|s_1\rangle=\begin{pmatrix}\cos(\theta_1/2)\\\sin(\theta_1/2)\exp(i\phi_1)\end{pmatrix},\quad
|s_2\rangle=\begin{pmatrix}\cos(\theta_2/2)\\\sin(\theta_2/2)\exp(i\phi_2)\end{pmatrix}
\end{equation*}

and
\begin{equation*}
|s\rangle=|s_1\rangle\otimes|s_2\rangle
\end{equation*}

Verify that
\begin{equation*}
\langle s|\mathbf S_1|s\rangle
=\frac{\hbar}{2}\begin{pmatrix}
\sin\theta_1\cos\phi_1\\
\sin\theta_1\sin\phi_1\\
\cos\theta_1
\end{pmatrix},\quad
\langle s|\mathbf S_2|s\rangle
=\frac{\hbar}{2}\begin{pmatrix}
\sin\theta_2\cos\phi_2\\
\sin\theta_2\sin\phi_2\\
\cos\theta_2
\end{pmatrix}
\end{equation*}

\end{document}

\bigskip
Verify that
\begin{align*}
(S_{1x}+S_{2x})|z_{++}\rangle&=\tfrac{\hbar}{2}|z_{-+}\rangle+\tfrac{\hbar}{2}|z_{+-}\rangle
\\
(S_{1x}+S_{2x})|z_{+-}\rangle&=\tfrac{\hbar}{2}|z_{--}\rangle+\tfrac{\hbar}{2}|z_{++}\rangle
\\
(S_{1x}+S_{2x})|z_{-+}\rangle&=\tfrac{\hbar}{2}|z_{++}\rangle+\tfrac{\hbar}{2}|z_{--}\rangle
\\
(S_{1x}+S_{2x})|z_{--}\rangle&=\tfrac{\hbar}{2}|z_{+-}\rangle+\tfrac{\hbar}{2}|z_{-+}\rangle
\\
\\
(S_{1y}+S_{2y})|z_{++}\rangle&=\tfrac{i\hbar}{2}|z_{-+}\rangle+\tfrac{i\hbar}{2}|z_{+-}\rangle
\\
(S_{1y}+S_{2y})|z_{+-}\rangle&=\tfrac{i\hbar}{2}|z_{--}\rangle-\tfrac{i\hbar}{2}|z_{++}\rangle
\\
(S_{1y}+S_{2y})|z_{-+}\rangle&=-\tfrac{i\hbar}{2}|z_{++}\rangle+\tfrac{i\hbar}{2}|z_{--}\rangle
\\
(S_{1y}+S_{2y})|z_{--}\rangle&=-\tfrac{i\hbar}{2}|z_{+-}\rangle-\tfrac{i\hbar}{2}|z_{-+}\rangle
\\
\\
(S_{1x}+S_{2x})|z_{++}\rangle&=\tfrac{\hbar}{2}|z_{++}\rangle+\tfrac{\hbar}{2}|z_{++}\rangle
\\
(S_{1x}+S_{2x})|z_{+-}\rangle&=\tfrac{\hbar}{2}|z_{+-}\rangle-\tfrac{\hbar}{2}|z_{+-}\rangle
\\
(S_{1x}+S_{2x})|z_{-+}\rangle&=-\tfrac{\hbar}{2}|z_{-+}\rangle+\tfrac{\hbar}{2}|z_{-+}\rangle
\\
(S_{1x}+S_{2x})|z_{--}\rangle&=-\tfrac{\hbar}{2}|z_{--}\rangle-\tfrac{\hbar}{2}|z_{--}\rangle
\end{align*}

\end{document}
