\input{preamble}

\FBOX{
2-2.
For a harmonic oscillator $L=(m/2)(\dot x^2-\omega^2x^2)$.
With $T$ equal to $t_b-t_a$, show that the classical action is
\begin{equation*}
S_{cl}=\frac{m\omega}{2\sin\omega T}
\left(\left(x_b^2+x_a^2\right)\cos\omega T-2x_bx_a\right)
\tag{2.9}
\end{equation*}
}

We will need equation (2.7) to determine the classical motion $x(t)$.
\begin{equation*}
\frac{d}{dt}\frac{\partial L}{\partial\dot x}=\frac{\partial L}{\partial x}
\tag{2.7}
\end{equation*}

For the Lagrangian $L$ given in problem 2-2 we have
\begin{equation*}
\frac{d}{dt}\left(\frac{\partial L}{\partial\dot x}\right)=m\ddot x\,, % comma
\quad
\frac{\partial L}{\partial x}=-m\omega^2x
\end{equation*}

By equation (2.7) we have for the classical acceleration $\ddot x(t)$
\begin{equation*}
\ddot x(t)=-\omega^2x
\tag{1}
\end{equation*}

The well-known solution to (1) is
\begin{equation*}
x(t)=A\sin(\omega t)+B\cos(\omega t)
\end{equation*}

We have the following boundary conditions.
\begin{equation*}
x(0)=x_a\,, % comma
\quad
x(T)=x_b
\end{equation*}

Solve for $B$.
\begin{equation*}
B=x(0)=x_a
\end{equation*}

For $x(T)$ we have
\begin{equation*}
x(T)=A\sin(\omega T)+B\cos(\omega T)
\end{equation*}

Solve for $A$.
\begin{equation*}
A=\frac{x(T)-B\cos(\omega T)}{\sin(\omega T)}=
\frac{x_b-x_a\cos(\omega T)}{\sin(\omega T)}
\end{equation*}

Hence the equation of motion is
\begin{equation*}
x(t)=\frac{x_b-x_a\cos(\omega T)}{\sin(\omega T)}\sin(\omega t)+x_a\cos(\omega t)
\tag{2}
\end{equation*}

Differentiate $x(t)$ to obtain velocity $\dot x(t)$.
\begin{equation*}
\dot x(t)=\frac{d}{dt}x(t)=
\omega\left(
\frac{x_b-x_a\cos(\omega T)}{\sin(\omega T)}\cos(\omega t)-x_a\sin(\omega t)
\right)
\tag{3}
\end{equation*}

Using the action integral
\begin{equation*}
S=\int_0^T L\,dt
\end{equation*}
we have for the classical action
\begin{align*}
S_{cl}&=\frac{m}{2}\int_0^T (\dot{x}^2-\omega^2 x^2)\,dt
\\[1ex]
&=\frac{m}{2}\left(
\int_0^T\dot{x}^2\,dt
-\int_0^T\omega^2x^2\,dt\right)
\end{align*}

Use integration by parts to solve the first integral.
Let
\begin{equation*}
u=\dot x,\quad v'=\dot x
\end{equation*}

so that
\begin{equation*}
u'=\ddot x,\quad v=x
\end{equation*}

The integral transforms as
\begin{align*}
\int_0^T \dot x^2\,dt
&=\int_0^T uv'\,dt
\\
&=[uv]_0^T
-\int_0^Tu'v\,dt
\\
&=\dot x(T)x(T)-\dot x(0)x(0)-\int_0^T\ddot xx\,dt
\end{align*}

Hence
\begin{equation*}
S_{cl}=\frac{m}{2}\left(
\dot x(T)x(T)-\dot x(0)x(0)-\int_0^T \ddot xx\,dt
-\int_0^T\omega^2x^2\,dt
\right)
\end{equation*}

The remaining integrals cancel by $\ddot x=-\omega^2x$ from equation (1) leaving
\begin{equation*}
S_{cl}=\frac{m}{2}\bigl(\dot x(T)x(T)-\dot x(0)x(0)\bigr)
\tag{4}
\end{equation*}

By evaluation of $x(t)$ and $\dot x(t)$ at $t=T$ and $t=0$ we have
\begin{equation*}
S_{cl}=\frac{m\omega}{2\sin(\omega T)}
\left(\left(x_b^2+x_a^2\right)\cos(\omega T)-2x_b x_a\right)
\tag{5}
\end{equation*}

\end{document}
